splitting: commit all work on FOL compactness

Splitting_Framework/FOL_Compactness.thy
@@ -3,23 +3,18 @@ theory FOL_Compactness
     Main
     HOL.Zorn
     Ordered_Resolution_Prover.Clausal_Logic
+    First_Order_Terms.Term
+    "HOL-Library.FuncSet"
+    "HOL-Library.Countable"
 begin
 
+(* TODO: Review the notations used!! *)
 
-(* A few notes:
- *
- * - There is an AFP entry named "FOL-Fitting", which models the full First-Order logic along with
- *   substitutions and a small natural deduction calculus.
- *   Unfortunately, this will not work for our purpose, as it uses lists internally, while we make
- *   use of (possibly) infinite sets.
- * - We could have used the AFP entry "First-order terms" instead of re-defining terms.
- *   However, we do not really need all the results about substitutions and unification. *)
 
 text \<open>
   On-going formalisation of ``Le nec plus ultra du théorème de compacité'' by Pierre Cagne.
 
-  Basically, we define a Tarski entailment, prove that it is compact, and provide a translation from
-  First-Order formulas in CNF to the @{typ \<open>_ clause\<close>} type.
+  Basically, we define a Tarski entailment and prove that it is compact.
 \<close>
 
 no_syntax
@@ -32,13 +27,12 @@ text \<open>
   \<^item> Variables of abstract type \<open>'v\<close>;
   \<^item> Constants of abstract type \<open>'c\<close>;
   \<^item> Or function applications on terms.
+
+  Note that our \<open>tm\<close> type models constants as 0-ary functions, i.e. \<open>c()\<close>.
 \<close> 
 
 (* Definition 1.1 *)
-datatype ('c, 'v) tm =
-  Var 'v
-| Const 'c
-| Fn 'v \<open>('c, 'v) tm list\<close>
+type_synonym ('f, 'v) tm = \<open>('f, 'v) term\<close> 
 
 text \<open>
   First-order formulas:
@@ -49,65 +43,339 @@ text \<open>
 \<close>
 
 (* Definition 1.2 *)
-datatype ('c, 'v) fm =
-  Rel 'v \<open>('c, 'v) tm list\<close>
-| Negation \<open>('c, 'v) fm\<close> (\<open>\<^bold>\<not> _\<close> [70] 70)
-| Conjunction \<open>('c, 'v) fm\<close> \<open>('c, 'v) fm\<close> (infixl \<open>\<^bold>\<and>\<close> 65)
-| Existential 'v \<open>('c, 'v) fm\<close> (\<open>\<^bold>\<exists> _\<^bold>. _\<close>)
-| Top (\<open>\<^bold>\<top>\<close>)
-| Bot (\<open>\<^bold>\<bottom>\<close>) 
+datatype ('f, 'p, 'v) fm =
+  Rel 'p \<open>('f, 'v) tm list\<close>
+| Negation \<open>('f, 'p, 'v) fm\<close> (\<open>\<^bold>\<not> _\<close> [90] 90)
+| Conjunction \<open>('f, 'p, 'v) fm\<close> \<open>('f, 'p, 'v) fm\<close> (infixl \<open>\<^bold>\<and>\<close> 85)
+| Existential 'v \<open>('f, 'p, 'v) fm\<close> (\<open>\<^bold>\<exists> _\<^bold>. _\<close> [0, 70] 70)
+| Bot (\<open>\<^bold>\<bottom>\<close>)
 
-fun is_atomic :: \<open>('c, 'v) fm \<Rightarrow> bool\<close> where
+fun is_atomic :: \<open>('f, 'p, 'v) fm \<Rightarrow> bool\<close> where
   \<open>is_atomic (Rel _ _) = True\<close>
-| \<open>is_atomic _ = False\<close> 
+| \<open>is_atomic _ = False\<close>
 
-syntax
-  "_FOL_Forall" :: \<open>'v \<Rightarrow> ('c, 'v) fm \<Rightarrow> ('c, 'v) fm\<close> (\<open>\<^bold>\<forall> _\<^bold>. _\<close>)
-  "_FOL_Disjunction" :: \<open>('c, 'v) fm \<Rightarrow> ('c, 'v) fm \<Rightarrow> ('c, 'v) fm\<close> (infixl \<open>\<^bold>\<or>\<close> 64)
-  "_FOL_Implication" :: \<open>('c, 'v) fm \<Rightarrow> ('c, 'v) fm \<Rightarrow> ('c, 'v) fm\<close> (infixr \<open>\<^bold>\<longrightarrow>\<close> 50)
-(*  "_FOL_Equivalence" :: \<open>('c, 'v) fm \<Rightarrow> ('c, 'v) fm \<Rightarrow> ('c, 'v) fm\<close> (\<open>_ \<^bold>\<longleftrightarrow> _\<close>) *) 
+text \<open>
+  Some input shortcuts (because we can). 
+\<close> 
 
-translations
-  "\<^bold>\<forall> x\<^bold>. \<phi>" \<rightleftharpoons> "\<^bold>\<exists> x\<^bold>. \<phi>"
-  "\<phi> \<^bold>\<or> \<psi>" \<rightleftharpoons> "\<^bold>\<not> (\<^bold>\<not> \<phi> \<^bold>\<and> \<^bold>\<not> \<psi>)"
-  "\<phi> \<^bold>\<longrightarrow> \<psi>" \<rightleftharpoons> "\<^bold>\<not> \<phi> \<^bold>\<or> \<psi>"
-(* NOTE: not permitted because of duplicated variables on the right-hand side.
- * But it's okay. We don't really care too much about equivalence.
- * If we really did, we would define it in the @{typ fm} datatype (same applies to all other
- * notations). *)
-(*  "\<phi> \<^bold>\<longleftrightarrow> \<psi>" \<rightleftharpoons> "(\<phi> \<^bold>\<longrightarrow> \<psi>) \<^bold>\<and> (\<psi> \<^bold>\<longrightarrow> \<phi>)" *) 
+abbreviation (input) Forall :: \<open>'v \<Rightarrow> ('f, 'p, 'v) fm \<Rightarrow> ('f, 'p, 'v) fm\<close> (\<open>\<^bold>\<forall> _\<^bold>. _\<close> [0, 70] 70) where
+  \<open>\<^bold>\<forall> x\<^bold>. \<phi> \<equiv> \<^bold>\<not> (\<^bold>\<exists> x\<^bold>. \<^bold>\<not> \<phi>)\<close>
+
+abbreviation (input) Disjunction :: \<open>('f, 'p, 'v) fm \<Rightarrow> ('f, 'p, 'v) fm \<Rightarrow> ('f, 'p, 'v) fm\<close>
+  (infixl \<open>\<^bold>\<or>\<close> 84) where
+  \<open>\<phi> \<^bold>\<or> \<psi> \<equiv> \<^bold>\<not> (\<^bold>\<not> \<phi> \<^bold>\<and> \<^bold>\<not> \<psi>)\<close>
+
+abbreviation (input) Implication :: \<open>('f, 'p, 'v) fm \<Rightarrow> ('f, 'p, 'v) fm \<Rightarrow> ('f, 'p, 'v) fm\<close>
+  (infixr \<open>\<^bold>\<longrightarrow>\<close> 70) where
+  \<open>\<phi> \<^bold>\<longrightarrow> \<psi> \<equiv> \<^bold>\<not> \<phi> \<^bold>\<or> \<psi>\<close>
+
+abbreviation (input) Equivalence :: \<open>('f, 'p, 'v) fm \<Rightarrow> ('f, 'p, 'v) fm \<Rightarrow> ('f, 'p, 'v) fm\<close>
+  (infix \<open>\<^bold>\<longleftrightarrow>\<close> 70) where
+  \<open>\<phi> \<^bold>\<longleftrightarrow> \<psi> \<equiv> (\<phi> \<^bold>\<longrightarrow> \<psi> \<^bold>\<and> \<psi> \<^bold>\<longrightarrow> \<phi>)\<close> 
+
+abbreviation (input) Top :: \<open>('f, 'p, 'v) fm\<close> (\<open>\<^bold>\<top>\<close>) where
+  \<open>\<^bold>\<top> \<equiv> \<^bold>\<not> \<^bold>\<bottom>\<close> 
 
 text \<open>
   We also define the notion of free and bound variables.
   A free variable occurrence is an occurrence not appearing in the scope of any quantifier.
   For example, the first occurrence of \<open>x\<close> in the formula \<open>(x \<^bold>\<doteq> y) \<^bold>\<longleftrightarrow> (\<^bold>\<exists> x\<^bold>. x \<^bold>\<doteq> y)\<close> is free, while
-  the second is bound.
+  the second is bound (assuming that a predicate \<open>\<^bold>\<doteq>\<close> of arity 2 is defined).
 \<close> 
 
-fun FV_tm :: \<open>('f, 'v) tm \<Rightarrow> 'v set\<close> where
-  \<open>FV_tm (Var v) = {v}\<close>
-| \<open>FV_tm (Const _) = {}\<close>
-| \<open>FV_tm (Fn _ args) = (\<Union> a \<in> set args. FV_tm a)\<close>
+fun size_fm :: \<open>('f, 'p, 'v) fm \<Rightarrow> nat\<close> where
+  \<open>size_fm \<^bold>\<bottom> = 1\<close>
+| \<open>size_fm (Rel p ts) = 1\<close>
+| \<open>size_fm (\<^bold>\<not> \<phi>) = 1 + size_fm \<phi>\<close>
+| \<open>size_fm (\<phi> \<^bold>\<and> \<psi>) = size_fm \<phi> + size_fm \<psi>\<close>
+| \<open>size_fm (\<^bold>\<exists> x\<^bold>. \<phi>) = 1 + size_fm \<phi>\<close> 
 
-fun FV_fm :: \<open>('f, 'v) fm \<Rightarrow> 'v set\<close> where
-  \<open>FV_fm (Rel _ args) = (\<Union> a \<in> set args. FV_tm a)\<close>
+lemma [measure_function]: \<open>is_measure size_fm\<close> ..
+
+abbreviation FV_tm :: \<open>('f, 'v) tm \<Rightarrow> 'v set\<close> where
+  \<open>FV_tm \<equiv> vars_term\<close>
+
+fun FV_fm :: \<open>('f, 'p, 'v) fm \<Rightarrow> 'v set\<close> where
+  \<open>FV_fm (Rel _ args') = (\<Union> a \<in> set args'. FV_tm a)\<close>
 | \<open>FV_fm (\<^bold>\<not> \<phi>) = FV_fm \<phi>\<close>
 | \<open>FV_fm (\<phi> \<^bold>\<and> \<psi>) = FV_fm \<phi> \<union> FV_fm \<psi>\<close>
 | \<open>FV_fm (\<^bold>\<exists> x\<^bold>. \<phi>) = FV_fm \<phi> - {x}\<close>
-| \<open>FV_fm \<^bold>\<top> = {}\<close>
-| \<open>FV_fm \<^bold>\<bottom> = {}\<close> 
-
-lemma finite_FV_tm: \<open>finite (FV_tm t)\<close>
-  by (induction t, auto) 
+| \<open>FV_fm \<^bold>\<bottom> = {}\<close>
 
 lemma finite_FV_fm: \<open>finite (FV_fm \<phi>)\<close>
-  by (induction \<phi>, auto simp add: finite_FV_tm) 
+  by (induction \<phi>, auto) 
 
-subsection \<open>Structures and Models\<close> 
+fun subst_fm :: \<open>('f, 'p, 'v) fm \<Rightarrow> ('f, 'v) subst \<Rightarrow> ('f, 'p, 'v) fm\<close> (infixl \<open>\<cdot>\<^sub>f\<^sub>m\<close> 75) where
+  \<open>\<^bold>\<bottom> \<cdot>\<^sub>f\<^sub>m _ = \<^bold>\<bottom>\<close> 
+| \<open>(Rel p ts) \<cdot>\<^sub>f\<^sub>m \<sigma> = Rel p [t \<cdot> \<sigma>. t \<leftarrow> ts]\<close>
+| \<open>(\<^bold>\<not> \<phi>) \<cdot>\<^sub>f\<^sub>m \<sigma> = \<^bold>\<not> (\<phi> \<cdot>\<^sub>f\<^sub>m \<sigma>)\<close>
+| \<open>(\<phi> \<^bold>\<and> \<psi>) \<cdot>\<^sub>f\<^sub>m \<sigma> = (\<phi> \<cdot>\<^sub>f\<^sub>m \<sigma>) \<^bold>\<and> (\<psi> \<cdot>\<^sub>f\<^sub>m \<sigma>)\<close>
+| \<open>(\<^bold>\<exists> x\<^bold>. \<phi>) \<cdot>\<^sub>f\<^sub>m \<sigma> =
+    (let \<sigma>' = \<sigma>(x := Var x);
+         z = if \<exists> y. y \<in> FV_fm (\<^bold>\<exists> x\<^bold>. \<phi>) \<and> x \<in> FV_tm (\<sigma>' y)
+             then (\<some> z. z \<notin> FV_fm (\<phi> \<cdot>\<^sub>f\<^sub>m \<sigma>')) else x in
+    \<^bold>\<exists> z\<^bold>. (\<phi> \<cdot>\<^sub>f\<^sub>m \<sigma>(x := Var z)))\<close> 
+
+lemma [termination_simp]: \<open>size_fm (subst_fm \<phi> \<sigma>) = size_fm \<phi>\<close>
+proof (induction \<phi> arbitrary: \<sigma>)
+  case (Existential x \<phi>)
+  then show ?case
+    by (metis (no_types, lifting) size_fm.simps(5) subst_fm.simps(5)) 
+qed auto
 
 text \<open>
-  A structure is a 4-uple containing:
-  \<^item> \<open>\<cdot>\<^sub>c\<^sup>M \<in> c \<rightarrow> M\<close>  is a function mapping constants to values in \<open>M\<close>;
+  A formula \<open>\<phi>\<close> is in Clausal Normal Form (CNF) if:
+  \<^item> it is the empty clause \<open>\<^bold>\<bottom>\<close>, or
+  \<^item> it is the application of a predicate, or
+  \<^item> it is the negation of the application of a predicate, or
+  \<^item> it is of the form \<open>\<psi> \<^bold>\<or> \<rho>\<close> where \<open>\<psi>\<close> and \<open>\<rho>\<close> are in CNF.
+\<close>
+
+fun is_cnf :: \<open>('f, 'p, 'v) fm \<Rightarrow> bool\<close> where
+  \<open>is_cnf (\<phi> \<^bold>\<or> \<psi>) \<longleftrightarrow> is_cnf \<phi> \<and> is_cnf \<psi>\<close>
+| \<open>is_cnf (Rel _ _) \<longleftrightarrow> True\<close>
+| \<open>is_cnf (\<^bold>\<not> Rel _ _) \<longleftrightarrow> True\<close>
+| \<open>is_cnf \<^bold>\<bottom> \<longleftrightarrow> True\<close>
+| \<open>is_cnf _ \<longleftrightarrow> False\<close>
+
+(* fun eq_upto_renaming :: \<open>('f, 'p, 'v) fm \<Rightarrow> ('f, 'p, 'v) fm \<Rightarrow> bool\<close> (infix \<open>\<equiv>\<^sub>R\<close> 50) where
+ *   \<open>\<^bold>\<bottom> \<equiv>\<^sub>R \<^bold>\<bottom> \<longleftrightarrow> True\<close>
+ * | \<open>Rel p ts \<equiv>\<^sub>R Rel p' ts' \<longleftrightarrow> p = p' \<and> ts = ts'\<close>
+ * | \<open>\<^bold>\<not> \<phi> \<equiv>\<^sub>R \<^bold>\<not> \<psi> \<longleftrightarrow> \<phi> \<equiv>\<^sub>R \<psi>\<close>
+ * | \<open>(\<phi> \<^bold>\<and> \<psi>) \<equiv>\<^sub>R (\<phi>' \<^bold>\<and> \<psi>') \<longleftrightarrow> \<phi> \<equiv>\<^sub>R \<phi>' \<and> \<psi> \<equiv>\<^sub>R \<psi>'\<close>
+ * | \<open>(\<^bold>\<exists> x\<^bold>. \<phi>) \<equiv>\<^sub>R (\<^bold>\<exists> y\<^bold>. \<psi>) \<longleftrightarrow>
+ *     (let z = \<some> z. z \<notin> FV_fm \<phi> \<union> FV_fm \<psi> in
+ *     (\<phi> \<cdot>\<^sub>f\<^sub>m subst x (Var z)) \<equiv>\<^sub>R (\<psi> \<cdot>\<^sub>f\<^sub>m subst y (Var z)))\<close>
+ * | \<open>_ \<equiv>\<^sub>R _ \<longleftrightarrow> False\<close> 
+ * 
+ * lemma neg_eq_rename_neg: 
+ *   assumes \<open>\<^bold>\<not> \<phi> \<equiv>\<^sub>R \<psi>\<close>
+ *   obtains \<rho> where
+ *     \<open>\<psi> = \<^bold>\<not> \<rho>\<close>
+ *   (\* Slow *\)
+ *   by (smt (verit) assms eq_upto_renaming.elims(1) fm.simps(14) fm.simps(16)) 
+ * 
+ * lemma subst_fm_x_x_is_fm: \<open>subst_fm \<phi> (subst x (Var x)) = \<phi>\<close>
+ *   by (induction \<phi>) auto
+ * 
+ * lemma subst_fm_var_not_in_FV: \<open>x \<notin> FV_fm \<phi> \<Longrightarrow> subst_fm \<phi> (subst x t) = \<phi>\<close> 
+ * proof (induction \<phi>)
+ *   case (Existential y \<phi>)
+ * 
+ *   consider
+ *     (a) \<open>x = y\<close>
+ *   | (b) \<open>x \<noteq> y\<close>
+ *     by blast 
+ *   then show ?case
+ *   proof (cases) 
+ *     case a
+ *     then show ?thesis
+ *       by (smt (verit, best) DiffD2 Diff_insert_absorb Existential.prems Term.term.simps(17)
+ *           fun_upd_upd insert_iff subst_def subst_fm.simps(5) subst_fm_x_x_is_fm subst_simps(2))
+ *   next
+ *     case b
+ *     then have \<open>x \<notin> FV_fm \<phi>\<close>
+ *       using Existential.prems
+ *       by simp 
+ *     then have \<open>subst_fm \<phi> (subst x t) = \<phi>\<close>
+ *       using Existential.IH
+ *       by auto 
+ *     then show ?thesis
+ *       by (smt (verit, del_insts) Diff_iff Existential.prems FV_fm.simps(4) Term.term.simps(17) b
+ *           fun_upd_other fun_upd_triv singleton_iff subst_def subst_fm.simps(5)) 
+ *   qed
+ * qed (auto simp add: list.map_ident_strong)
+ * 
+ * (\* lemma \<open>subst_fm (subst_fm \<phi> \<sigma>) \<rho> \<equiv>\<^sub>R subst_fm \<phi> (\<sigma> \<circ>\<^sub>s \<rho>)\<close>
+ * proof (induction \<phi>)
+ *   case (Existential x \<phi>)
+ *   then show ?case
+ *     apply auto
+ *      
+ *     sorry
+ * qed auto
+ * 
+ * lemma \<open>\<phi> \<equiv>\<^sub>R \<psi> \<Longrightarrow> subst_fm \<phi> \<sigma> \<equiv>\<^sub>R subst_fm \<psi> \<sigma>\<close>
+ * proof (induction \<phi> \<psi> rule: eq_upto_renaming.induct)
+ *   case (5 x \<phi> y \<psi>)
+ *   then show ?case
+ *     apply auto
+ *     subgoal sorry
+ *     subgoal sorry
+ *     subgoal sorry 
+ *     sorry
+ * qed (simp; meson eq_upto_renaming.simps)+
+ * (\* Some subgoals are discharged already by \<open>simp\<close>. In those cases, we do not want to apply \<open>meson\<close>
+ *  * at all. \<open>;\<close> allows us to do just that (because it tries to iterate an empty list of subgoals).
+ *  * Alternatively, I think that just \<open>meson eq_upto_renaming.simps subst_fm.simps\<close> should work just
+ *  * fine, but I did not test it. *\) *\)
+ * 
+ * lemma apply_subst_term_upd_cancel:
+ *   assumes \<open>y \<notin> FV_tm t\<close>
+ *   shows \<open>t \<cdot> \<sigma>(y := t') = t \<cdot> \<sigma>\<close>
+ *   by (simp add: assms term_subst_eq_conv) 
+ * 
+ * lemma apply_subst_term_chain_upd_cancel:
+ *   assumes \<open>y \<notin> FV_tm t\<close>
+ *   shows \<open>t' \<cdot> subst y t \<cdot> \<sigma>(y := Var y) = t' \<cdot> subst y t \<cdot> \<sigma>\<close>
+ *   using assms
+ * proof (induction t') 
+ *   case (Var v)
+ * 
+ *   show ?case
+ *     unfolding subst_def
+ *     by (metis assms fun_upd_other fun_upd_same subst_apply_term.simps(1) term_subst_eq) 
+ * next
+ *   case (Fun f ts)
+ *   then show ?case
+ *     by auto
+ * qed
+ * 
+ * lemma \<open>FV_fm (\<phi> \<cdot>\<^sub>f\<^sub>m \<sigma>) = \<Union> (FV_tm ` \<sigma> ` FV_fm \<phi>)\<close>
+ * proof (induction \<phi> arbitrary: \<sigma>)
+ *   case (Rel p ts)
+ *   then show ?case
+ *     by (simp add: vars_term_subst) 
+ * next
+ *   case (Existential x \<phi>)
+ *   then show ?case
+ *      
+ *     sorry
+ * qed auto 
+ * 
+ * lemma
+ *   assumes \<open>y \<notin> FV_tm t\<close>
+ *   shows \<open>\<phi> \<cdot>\<^sub>f\<^sub>m subst y t \<cdot>\<^sub>f\<^sub>m \<sigma>(y := Var y) \<equiv>\<^sub>R \<phi> \<cdot>\<^sub>f\<^sub>m subst y t \<cdot>\<^sub>f\<^sub>m \<sigma>\<close>
+ *   using assms
+ * proof (induction \<phi>) 
+ *   case (Rel p ts)
+ * 
+ *   show ?case
+ *     using apply_subst_term_chain_upd_cancel[OF Rel.prems(1), of _ \<sigma>]
+ *     by auto (smt (verit, best) fun_upd_same term_subst_eq term_subst_eq_rev) 
+ * next
+ *   case (Existential x \<phi>)
+ *   then show ?case
+ *     apply auto
+ *      
+ *     sorry
+ * qed auto *)
+
+context
+  assumes UNIV_contains_all_vars: \<open>\<forall> \<phi> :: ('f, 'p, 'v) fm. FV_fm \<phi> \<subset> UNIV\<close>
+begin
+
+lemma ex_fresh_var:
+  fixes \<phi> :: \<open>('f, 'p, 'v) fm\<close> 
+  obtains v where
+    \<open>v \<notin> FV_fm \<phi>\<close>
+  using UNIV_contains_all_vars
+  by blast
+
+end (* context *)
+
+definition is_ground_tm :: \<open>('f, 'v) tm \<Rightarrow> bool\<close> where
+  \<open>is_ground_tm t \<equiv> \<forall> \<sigma>. t \<cdot> \<sigma> = t\<close>
+
+definition is_ground_subst :: \<open>('f, 'v) subst \<Rightarrow> bool\<close> where
+  \<open>is_ground_subst \<sigma> \<equiv> \<forall> t. is_ground_tm (t \<cdot> \<sigma>)\<close> 
+
+lemma tm_is_ground_iff_closed: \<open>is_ground_tm t \<longleftrightarrow> FV_tm t = {}\<close>
+proof (induction t) 
+  case (Var v)
+
+  have \<open>\<not> is_ground_tm (Var v)\<close>
+    unfolding is_ground_tm_def
+    by auto 
+  moreover have \<open>FV_tm (Var v) \<noteq> {}\<close>
+    by auto 
+  ultimately show ?case
+    by blast
+next
+  case (Fun f ts)
+
+  have \<open>\<forall> t \<in> set ts. is_ground_tm t \<longleftrightarrow> FV_tm t = {}\<close>
+    using Fun.IH
+    by (intro ballI)
+  moreover have \<open>\<forall> \<sigma>. (Fun f ts) \<cdot> \<sigma> = Fun f [t \<cdot> \<sigma>. t \<leftarrow> ts]\<close>
+    by auto 
+  ultimately have \<open>(\<forall> \<sigma>. Fun f [t \<cdot> \<sigma>. t \<leftarrow> ts] = Fun f ts) \<longleftrightarrow> FV_tm (Fun f ts) = {}\<close>
+    unfolding is_ground_tm_def
+    (* Slow-ish *)
+    by (smt (z3) empty_iff equals0I subst_apply_term.simps(2) subst_apply_term_empty subst_ident
+        subst_simps(1) term.distinct(1) term.inject(2) term_subst_eq term_subst_eq_rev) 
+  then show ?case
+    unfolding is_ground_tm_def
+    by auto 
+qed
+
+lemma ground_tm_subst: \<open>is_ground_tm t \<Longrightarrow> t \<cdot> \<sigma> = t\<close>
+  unfolding is_ground_tm_def
+  by blast
+
+lemma subst_term_ground_subst_is_ground: \<open>is_ground_subst \<sigma> \<Longrightarrow> is_ground_tm (t \<cdot> \<sigma>)\<close>
+  unfolding is_ground_subst_def
+  by blast
+
+text \<open>
+  The grounding function \<open>\<G>\<close> returns all ground instances of a set of formulas.
+\<close> 
+
+abbreviation \<open>\<G> N \<equiv> \<Union> \<phi> \<in> N. {\<phi> \<cdot>\<^sub>f\<^sub>m \<sigma> | \<sigma>. is_ground_subst \<sigma>}\<close> 
+
+lemma ex_ground_subst: \<open>\<exists> \<sigma> :: ('f, 'v) subst. is_ground_subst \<sigma>\<close>
+  unfolding is_ground_subst_def
+proof -
+  obtain f :: 'f and \<sigma> :: \<open>('f, 'v) subst\<close> where
+    \<open>\<forall> v. \<sigma> v = Fun f []\<close>
+    by force
+  moreover have \<open>is_ground_tm (Fun f [])\<close>
+    unfolding is_ground_tm_def
+    by simp 
+  ultimately have \<open>is_ground_tm (t \<cdot> \<sigma>)\<close>
+    for t
+    unfolding is_ground_tm_def
+    by (induction t, auto)
+  then have \<open>\<forall> t. is_ground_tm (t \<cdot> \<sigma>)\<close>
+    by blast 
+  then show \<open>\<exists> \<sigma> :: ('f, 'v) subst. \<forall> t. is_ground_tm (t \<cdot> \<sigma>)\<close>
+    by blast 
+qed 
+
+text \<open>
+  Extract the language \<open>\<L>\<close> used in the formula.
+  Function (and predicate) symbols are bundled together with their respective arities.
+\<close> 
+
+fun fn_sym_tm :: \<open>('f, 'v) tm \<Rightarrow> ('f \<times> nat) set\<close> where
+  \<open>fn_sym_tm (Var _) = {}\<close>
+| \<open>fn_sym_tm (Fun f ts) = {(f, length ts)} \<union> (\<Union> t \<in> set ts. fn_sym_tm t)\<close>
+
+fun fn_sym_fm :: \<open>('f, 'p, 'v) fm \<Rightarrow> ('f \<times> nat) set\<close> where
+  \<open>fn_sym_fm \<^bold>\<bottom> = {}\<close>
+| \<open>fn_sym_fm (\<phi> \<^bold>\<and> \<psi>) = fn_sym_fm \<phi> \<union> fn_sym_fm \<psi>\<close>
+| \<open>fn_sym_fm (\<^bold>\<not> \<phi>) = fn_sym_fm \<phi>\<close>
+| \<open>fn_sym_fm (\<^bold>\<exists> x\<^bold>. \<phi>) = fn_sym_fm \<phi>\<close>
+| \<open>fn_sym_fm (Rel p ts) = (\<Union> t \<in> set ts. fn_sym_tm t)\<close> 
+
+fun pred_sym_fm :: \<open>('f, 'p, 'v) fm \<Rightarrow> ('p \<times> nat) set\<close> where
+  \<open>pred_sym_fm \<^bold>\<bottom> = {}\<close>
+| \<open>pred_sym_fm (\<phi> \<^bold>\<and> \<psi>) = pred_sym_fm \<phi> \<union> pred_sym_fm \<psi>\<close>
+| \<open>pred_sym_fm (\<^bold>\<not> \<phi>) = pred_sym_fm \<phi>\<close>
+| \<open>pred_sym_fm (\<^bold>\<exists> x\<^bold>. \<phi>) = pred_sym_fm \<phi>\<close>
+| \<open>pred_sym_fm (Rel p ts) = {(p, length ts)}\<close>
+
+abbreviation \<open>language S \<equiv> (\<Union> \<phi> \<in> S. fn_sym_fm \<phi>, \<Union> \<phi> \<in> S. pred_sym_fm \<phi>)\<close> 
+
+inductive_set terms :: \<open>('f \<times> nat) set \<times> ('p \<times> nat) set \<Rightarrow> ('f, 'v) tm set\<close>
+  for \<L> :: \<open>('f \<times> nat) set \<times> ('p \<times> nat) set\<close> where
+  var: \<open>Var (v :: 'v) \<in> terms \<L>\<close>
+| fn: \<open>(f, length ts) \<in> fst \<L> \<Longrightarrow> list_all (\<lambda> t. t \<in> terms \<L>) ts \<Longrightarrow> Fun f ts \<in> terms \<L>\<close> 
+  
+subsection \<open>Structures and Models\<close>
+
+text \<open>
+  A structure is a 3-uple containing:
   \<^item> \<open>\<cdot>\<^sub>f\<^sup>M \<in> M\<^sup>n \<rightarrow> M\<close> is a function mapping function symbols to functions from \<open>M\<^sup>n\<close> to \<open>M\<close>;
   \<^item> \<open>\<cdot>\<^sub>v\<^sup>M \<in> V \<rightarrow> M\<close> is a function mapping (free) variable symbols to values of \<open>M\<close>;
   \<^item> \<open>\<cdot>\<^sub>r\<^sup>M \<in> M\<^sup>n \<rightarrow> \<bool>\<close> (which we could also write \<open>\<cdot>\<^sub>r\<^sup>M \<subseteq> M\<^sup>n\<close>) is a function (relation) mapping values
@@ -115,39 +383,220 @@ text \<open>
 \<close> 
 
 (* Definition 1.3 *)
-record ('c, 'v, 'm) interp =
-  interp_const :: \<open>'c \<Rightarrow> 'm\<close> (\<open>CST\<close>)
-  interp_var :: \<open>'v \<Rightarrow> 'm\<close> (\<open>VAR\<close>)
-  interp_fun :: \<open>'v \<Rightarrow> 'm list \<Rightarrow> 'm\<close> (\<open>FN\<close>)
-  interp_rel :: \<open>'v \<Rightarrow> 'm list \<Rightarrow> bool\<close> (\<open>REL\<close>)
-  
-definition bind_var :: \<open>'v \<Rightarrow> 'm \<Rightarrow> ('c, 'v, 'm) interp \<Rightarrow> ('c, 'v, 'm) interp\<close> where
-  \<open>bind_var x y \<M> \<equiv> \<M>\<lparr> interp_var := (\<lambda> z. if x = z then y else VAR \<M> z) \<rparr>\<close> 
+locale struct =
+  fixes
+    M :: \<open>'m set\<close> and
+    FN :: \<open>'f \<Rightarrow> 'm list \<Rightarrow> 'm\<close> and
+    REL :: \<open>'p \<Rightarrow> 'm list set\<close> 
+  assumes
+    M_nonempty: \<open>M \<noteq> {}\<close> and 
+    FN_dom_to_dom: \<open>\<forall> f es. (\<forall> e \<in> set es. e \<in> M) \<longrightarrow> FN f es \<in> M\<close> and
+    REL_to_dom: \<open>\<forall> p. \<forall> es \<in> REL p. \<forall> e \<in> set es. e \<in> M\<close> 
 
-syntax
-  "_Bind_var" :: \<open>('c, 'v, 'm) interp \<Rightarrow> 'v \<Rightarrow> 'm \<Rightarrow> ('c, 'v, 'm) interp\<close> (\<open>_/'(_ \<mapsto> _')\<close> [80, 50, 50] 80)
+definition is_vars :: \<open>'m set \<Rightarrow> ('v \<Rightarrow> 'm) \<Rightarrow> bool\<close> where
+  [simp]: \<open>is_vars M \<beta> \<longleftrightarrow> (\<forall> v. \<beta> v \<in> M)\<close> 
 
-translations
-  "\<M>(x \<mapsto> v)" \<rightleftharpoons> "CONST bind_var x v \<M>"
+text \<open>
+  We are only interested in domains which are countable.
+\<close> 
+
+typedef ('f, 'p, 'm) model =
+  \<open>{ (M :: 'm set, FN :: 'f \<Rightarrow> 'm list \<Rightarrow> 'm, REL :: 'p \<Rightarrow> 'm list set). struct M FN REL }\<close>
+  using struct.intro
+  by fastforce
+
+setup_lifting type_definition_model
+
+lift_definition dom :: \<open>('f, 'p, 'm) model \<Rightarrow> 'm set\<close> is fst .
+lift_definition interp_fn :: \<open>('f, 'p, 'm) model \<Rightarrow> ('f \<Rightarrow> 'm list \<Rightarrow> 'm)\<close> is \<open>fst \<circ> snd\<close> .
+lift_definition interp_rel :: \<open>('f, 'p, 'm) model \<Rightarrow> ('p \<Rightarrow> 'm list set)\<close> is \<open>snd \<circ> snd\<close> .
+
+lemma model_is_struct: \<open>struct (dom \<M>) (interp_fn \<M>) (interp_rel \<M>)\<close>
+  by transfer auto 
+
+lemma dom_Abs_is_fst [simp]: \<open>struct M FN REL \<Longrightarrow> dom (Abs_model (M, FN, REL)) = M\<close>
+  by (simp add: Abs_model_inverse dom.rep_eq) 
+
+lemma interp_fn_Abs_is_fst_snd [simp]: \<open>struct M FN REL \<Longrightarrow> interp_fn (Abs_model (M, FN, REL)) = FN\<close>
+  by (simp add: Abs_model_inverse interp_fn.rep_eq) 
+
+lemma interp_rel_Abs_is_snd_snd [simp]: \<open>struct M FN REL \<Longrightarrow> interp_rel (Abs_model (M, FN, REL)) = REL\<close>
+  by (simp add: Abs_model_inverse interp_rel.rep_eq) 
+
+lemma FN_dom_to_dom: \<open>\<forall> t \<in> set ts. t \<in> dom \<M> \<Longrightarrow> interp_fn \<M> f ts \<in> dom \<M>\<close>
+  by (meson model_is_struct struct.FN_dom_to_dom)  
+
+text \<open>
+  We use canonical models to prove (un-)satisfiability.
+
+  A canonical model is a model whose domain is the set of terms and where function symbols are
+  interpreted as ``themselves'' (i.e. \<open>\<lbrakk>f(t\<^sub>1, \<dots>, t\<^sub>n)\<rbrakk>\<^bsup>\<J>,\<beta>\<^esup> = f(\<lbrakk>t\<^sub>1\<rbrakk>\<^bsup>\<J>,\<beta>\<^esup>, \<dots>, \<lbrakk>t\<^sub>n\<rbrakk>\<^bsup>\<J>,\<beta>\<^esup>)\<close>).
+  This is also refered to as ``Herbrand models'' in the literature.
+\<close> 
+
+definition is_canonical
+  :: \<open>('f, 'p, ('f, 'v) tm) model \<Rightarrow> ('f \<times> nat) set \<times> ('p \<times> nat) set \<Rightarrow> bool\<close> where
+  \<open>is_canonical \<M> \<L> \<longleftrightarrow> dom \<M> = terms \<L> \<and> interp_fn \<M> = Fun\<close> 
 
 text \<open>
   We define the notion of satisfaction inductively on formulas, and evaluation on terms.
 \<close>
 
-fun eval :: \<open>('c, 'v) tm \<Rightarrow> ('c, 'v, 'm) interp \<Rightarrow> 'm\<close> (\<open>_\<^sup>_\<close>) where
-  \<open>(Var v)\<^sup>\<M> = VAR \<M> v\<close>
-| \<open>(Fn f args)\<^sup>\<M> = FN \<M> f [t\<^sup>\<M>. t \<leftarrow> args]\<close> 
-| \<open>(Const c)\<^sup>\<M> = CST \<M> c\<close> 
-
-fun satisfies :: \<open>('c, 'v, 'm) interp \<Rightarrow> ('c, 'v) fm \<Rightarrow> bool\<close> (infix \<open>\<turnstile>\<close> 60) where
-  \<open>\<M> \<turnstile> \<^bold>\<top> = True\<close>
-| \<open>\<M> \<turnstile> \<^bold>\<bottom> = False\<close>
-| \<open>\<M> \<turnstile> \<^bold>\<not> \<phi> = (\<not> \<M> \<turnstile> \<phi>)\<close>
-| \<open>\<M> \<turnstile> \<phi> \<^bold>\<and> \<psi> = (\<M> \<turnstile> \<phi> \<and> \<M> \<turnstile> \<psi>)\<close>
-| \<open>\<M> \<turnstile> (\<^bold>\<exists> x\<^bold>. \<phi>) = (\<exists> y :: 'm. \<M>(x \<mapsto> y) \<turnstile> \<phi>)\<close>
-| \<open>\<M> \<turnstile> Rel p args = REL \<M> p [t\<^sup>\<M>. t \<leftarrow> args]\<close> 
+fun eval
+  :: \<open>('f, 'v) tm \<Rightarrow> ('f, 'p, 'm) model \<Rightarrow> ('v \<Rightarrow> 'm) \<Rightarrow> 'm\<close>
+  (\<open>\<lbrakk>_\<rbrakk>\<^bsup>_,_\<^esup>\<close> [50, 0, 0] 70) where
+  \<open>\<lbrakk>Var v\<rbrakk>\<^bsup>_,\<beta>\<^esup> = \<beta> v\<close>
+| \<open>\<lbrakk>Fun f args'\<rbrakk>\<^bsup>\<M>,\<beta>\<^esup> = interp_fn \<M> f [\<lbrakk>t\<rbrakk>\<^bsup>\<M>,\<beta>\<^esup>. t \<leftarrow> args']\<close> 
 
 
+fun satisfies
+  :: \<open>('f, 'p, 'm) model \<Rightarrow> ('v \<Rightarrow> 'm) \<Rightarrow> ('f, 'p, 'v) fm \<Rightarrow> bool\<close>
+  (\<open>_,_ \<Turnstile> _\<close> [30, 30, 80] 80) where
+  \<open>\<M>,\<beta> \<Turnstile> \<^bold>\<bottom> \<longleftrightarrow> False\<close>
+| \<open>\<M>,\<beta> \<Turnstile> \<^bold>\<not> \<phi> \<longleftrightarrow> (\<not> (\<M>,\<beta> \<Turnstile> \<phi>))\<close>
+| \<open>\<M>,\<beta> \<Turnstile> \<phi> \<^bold>\<and> \<psi> \<longleftrightarrow> (\<M>,\<beta> \<Turnstile> \<phi>) \<and> (\<M>,\<beta> \<Turnstile> \<psi>)\<close>
+| \<open>\<M>,\<beta> \<Turnstile> (\<^bold>\<exists> x\<^bold>. \<phi>) \<longleftrightarrow> (\<exists> y \<in> dom \<M>. \<M>,\<beta>(x := y) \<Turnstile> \<phi>)\<close>
+| \<open>\<M>,\<beta> \<Turnstile> Rel p args' \<longleftrightarrow> [\<lbrakk>t\<rbrakk>\<^bsup>\<M>,\<beta>\<^esup>. t \<leftarrow> args'] \<in> interp_rel \<M> p\<close> 
+
+lemma satisfies_indep_\<beta>_if:
+  \<open>\<forall> v \<in> FV_fm \<phi>. \<beta>\<^sub>1 v = \<beta>\<^sub>2 v \<Longrightarrow> \<M>,\<beta>\<^sub>1 \<Turnstile> \<phi> \<longleftrightarrow> \<M>,\<beta>\<^sub>2 \<Turnstile> \<phi>\<close>
+proof (induction \<phi> arbitrary: \<beta>\<^sub>1 \<beta>\<^sub>2)
+  case (Rel p ts)
+  then have \<open>\<forall> t \<in> set ts. \<forall> v \<in> FV_tm t. \<beta>\<^sub>1 v = \<beta>\<^sub>2 v\<close>
+    by simp 
+  then have \<open>[\<lbrakk>t\<rbrakk>\<^bsup>\<M>,\<beta>\<^sub>1\<^esup>. t \<leftarrow> ts] = [\<lbrakk>t\<rbrakk>\<^bsup>\<M>,\<beta>\<^sub>2\<^esup>. t \<leftarrow> ts]\<close>
+  proof (induction ts) 
+    case Nil
+    then show ?case
+      by simp 
+  next
+    case (Cons a ts)
+    then show ?case
+    proof (induction a) 
+      case (Var x)
+      then show ?case
+        by simp 
+    next
+      case (Fun f ts')
+      then have \<open>\<forall> t \<in> set ts'. \<forall> v \<in> FV_tm t. \<beta>\<^sub>1 v = \<beta>\<^sub>2 v\<close>
+        by simp 
+      then have \<open>[\<lbrakk>t\<rbrakk>\<^bsup>\<M>,\<beta>\<^sub>1\<^esup>. t \<leftarrow> ts'] = [\<lbrakk>t\<rbrakk>\<^bsup>\<M>,\<beta>\<^sub>2\<^esup>. t \<leftarrow> ts']\<close>
+        using Cons.IH Fun.IH Fun.prems(2)
+        by force
+      then have \<open>interp_fn \<M> f [\<lbrakk>t\<rbrakk>\<^bsup>\<M>,\<beta>\<^sub>1\<^esup>. t \<leftarrow> ts'] = interp_fn \<M> f [\<lbrakk>t\<rbrakk>\<^bsup>\<M>,\<beta>\<^sub>2\<^esup>. t \<leftarrow> ts']\<close>
+        by argo 
+      then show ?case
+        using Cons.IH Fun.prems(2)
+        by force 
+    qed
+  qed
+  then have \<open>[\<lbrakk>t\<rbrakk>\<^bsup>\<M>,\<beta>\<^sub>1\<^esup>. t \<leftarrow> ts] \<in> interp_rel \<M> p \<longleftrightarrow> [\<lbrakk>t\<rbrakk>\<^bsup>\<M>,\<beta>\<^sub>2\<^esup>. t \<leftarrow> ts] \<in> interp_rel \<M> p\<close>
+    by argo 
+  then show ?case
+    by auto 
+next
+  case (Conjunction \<phi> \<psi>)
+  then have
+    \<open>\<forall> v \<in> FV_fm \<phi>. \<beta>\<^sub>1 v = \<beta>\<^sub>2 v\<close> and
+    \<open>\<forall> v \<in> FV_fm \<psi>. \<beta>\<^sub>1 v = \<beta>\<^sub>2 v\<close>
+    by auto
+  then have
+    \<open>\<M>,\<beta>\<^sub>1 \<Turnstile> \<phi> \<longleftrightarrow> \<M>,\<beta>\<^sub>2 \<Turnstile> \<phi>\<close> and
+    \<open>\<M>,\<beta>\<^sub>1 \<Turnstile> \<psi> \<longleftrightarrow> \<M>,\<beta>\<^sub>2 \<Turnstile> \<psi>\<close>
+    using Conjunction.IH
+    by auto
+  then show ?case
+    by simp 
+next
+  case (Existential x \<phi>)
+
+  show ?case (is \<open>?lhs \<longleftrightarrow> ?rhs\<close>)
+  proof (intro iffI)
+    assume ?lhs
+    then obtain a where
+      a_in_M: \<open>a \<in> dom \<M>\<close> and
+      \<open>\<M>,\<beta>\<^sub>1(x := a) \<Turnstile> \<phi>\<close>
+      by auto
+    then have \<open>\<M>,\<beta>\<^sub>2(x := a) \<Turnstile> \<phi>\<close>
+      using Existential.IH Existential.prems
+      by (smt (verit, best) DiffI FV_fm.simps(4) empty_iff fun_upd_apply insert_iff) 
+    then show ?rhs
+      using a_in_M
+      by auto 
+  next
+    assume ?rhs
+    then obtain a where
+      a_in_M: \<open>a \<in> dom \<M>\<close> and
+      \<open>\<M>,\<beta>\<^sub>2(x := a) \<Turnstile> \<phi>\<close>
+      by auto
+    then have \<open>\<M>,\<beta>\<^sub>1(x := a) \<Turnstile> \<phi>\<close>
+      using Existential.IH Existential.prems
+      by (smt (verit, best) DiffI FV_fm.simps(4) empty_iff fun_upd_apply insert_iff) 
+    then show ?lhs
+      using a_in_M
+      by auto
+  qed
+qed auto 
+
+lemma satisfies_indep_model_if:
+  fixes
+    \<phi> :: \<open>('f, 'p, 'v) fm\<close> and
+    \<M> \<M>' :: \<open>('f, 'p, 'm) model\<close> 
+  assumes
+    dom_eq: \<open>dom \<M> = dom \<M>'\<close> and
+    rel_eq: \<open>\<forall> p. interp_rel \<M> p = interp_rel \<M>' p\<close> and
+    fn_eq: \<open>\<forall> f ts. (f, length ts) \<in> fn_sym_fm \<phi> \<longrightarrow> interp_fn \<M> f ts = interp_fn \<M>' f ts\<close>
+  shows
+    \<open>\<forall> \<beta>. is_vars (dom \<M>) \<beta> \<longrightarrow> \<M>,\<beta> \<Turnstile> \<phi> \<longleftrightarrow> \<M>',\<beta> \<Turnstile> \<phi>\<close>
+  using fn_eq
+proof (intro allI impI, induction \<phi>)
+  case (Rel p ts)
+
+  have all_fn_sym_in: \<open>(\<Union> t \<in> set ts. fn_sym_tm t) \<subseteq> fn_sym_fm (Rel p ts)\<close> (is \<open>?A \<subseteq> _\<close>)
+    by simp 
+
+  have eval_tm_eq: \<open>\<lbrakk>t\<rbrakk>\<^bsup>\<M>,\<beta>\<^esup> = \<lbrakk>t\<rbrakk>\<^bsup>\<M>',\<beta>\<^esup>\<close>
+    if \<open>fn_sym_tm t \<subseteq> fn_sym_fm (Rel p ts)\<close> 
+    for t 
+    using that
+  proof (induction t) 
+    case (Fun f ts') 
+
+    have \<open>\<forall> t' \<in> set ts'. fn_sym_tm t' \<subseteq> fn_sym_fm (Rel p ts)\<close>
+      using Fun.prems
+      by auto
+    moreover have \<open>(f, length [\<lbrakk>t'\<rbrakk>\<^bsup>\<M>,\<beta>\<^esup>. t' \<leftarrow> ts']) \<in> fn_sym_fm (Rel p ts)\<close>
+      using Fun.prems
+      by fastforce 
+    ultimately show ?case
+      using Fun.IH Rel.prems(1)[rule_format, of f \<open>[\<lbrakk>t'\<rbrakk>\<^bsup>\<M>,\<beta>\<^esup>. t' \<leftarrow> ts']\<close>] 
+      by (smt (verit, del_insts) eval.simps(2) map_eq_conv)
+  qed auto 
+
+  have \<open>\<M>,\<beta> \<Turnstile> Rel p ts \<longleftrightarrow> [\<lbrakk>t\<rbrakk>\<^bsup>\<M>,\<beta>\<^esup>. t \<leftarrow> ts] \<in> interp_rel \<M> p\<close>
+    by simp
+  also have \<open>... \<longleftrightarrow> [\<lbrakk>t\<rbrakk>\<^bsup>\<M>,\<beta>\<^esup>. t \<leftarrow> ts] \<in> interp_rel \<M>' p\<close>
+    by (simp add: rel_eq)
+  also have \<open>... \<longleftrightarrow> [\<lbrakk>t\<rbrakk>\<^bsup>\<M>',\<beta>\<^esup>. t \<leftarrow> ts] \<in> interp_rel \<M>' p\<close>
+    using eval_tm_eq all_fn_sym_in
+    by (metis (mono_tags, lifting) UN_subset_iff map_eq_conv)
+  also have \<open>... \<longleftrightarrow> \<M>',\<beta> \<Turnstile> Rel p ts\<close>
+    by auto 
+  finally show ?case .
+next
+  case (Existential x \<phi>)
+
+  have \<open>\<M>,\<beta> \<Turnstile> (\<^bold>\<exists> x\<^bold>. \<phi>) \<longleftrightarrow> (\<exists> a \<in> dom \<M>. \<M>,\<beta>(x := a) \<Turnstile> \<phi>)\<close>
+    by simp 
+  also have \<open>... = (\<exists> a \<in> dom \<M>. \<M>',\<beta>(x := a) \<Turnstile> \<phi>)\<close>
+    using Existential.IH Existential.prems
+    by fastforce
+  also have \<open>... = (\<exists> a \<in> dom \<M>'. \<M>',\<beta>(x := a) \<Turnstile> \<phi>)\<close>
+    by (simp add: dom_eq)
+  also have \<open>... = \<M>',\<beta> \<Turnstile> (\<^bold>\<exists> x\<^bold>. \<phi>)\<close>
+    by auto 
+  finally show ?case . 
+qed auto
 
 
 (* text \<open>
@@ -170,57 +619,590 @@ lemma models_subsets: \<open>M \<subseteq> M' \<Longrightarrow> \<M>, M \<turnst
   by blast 
 
 lemma \<open>\<M>, M \<turnstile> C \<longleftrightarrow> \<M>, M \<union> {\<^bold>\<not> C} \<turnstile> \<^bold>\<bottom>\<close>
-  by auto *) 
+  by auto *)  
 
 text \<open>
-  A statement is a formula with no free variable.
-\<close> 
-
-typedef ('c, 'v) statement = \<open>{ \<phi> :: ('c, 'v) fm. FV_fm \<phi> = {} }\<close>
-  morphisms fm_of of_fm 
-  using FV_fm.simps(5)
-  by blast
-
-text \<open>
-  A theory is simply a set of statements.
-\<close> 
-
-type_synonym ('c, 'v) th = \<open>('c, 'v) statement set\<close>    
-
-text \<open>
-  An interpretation \<open>\<M>\<close> is a model of a theory \<open>T\<close> if every statement of \<open>T\<close> is satisfied by \<open>\<M>\<close>.
+  An interpretation \<open>\<M>\<close> is a model of a set of formulas \<open>T\<close> if every formula of \<open>T\<close> is satisfied by
+  \<open>\<M>\<close> (under any valuation).
 \<close> 
 
 (* Definition 1.5 *)
-definition is_model_of :: \<open>('c, 'v, 'm) interp \<Rightarrow> ('c, 'v) th \<Rightarrow> bool\<close> where
-  \<open>is_model_of \<M> T \<longleftrightarrow> (\<forall> \<phi> \<in> T. \<M> \<turnstile> fm_of \<phi>)\<close>
+definition is_model_of
+  :: \<open>('f, 'p, 'm) model \<Rightarrow> ('f, 'p, 'v) fm set \<Rightarrow> bool\<close>
+  where
+  \<open>is_model_of \<M> T \<longleftrightarrow> (\<forall> \<phi> \<in> T. \<forall> V. is_vars (dom \<M>) V \<longrightarrow> \<M>,V \<Turnstile> \<phi>)\<close>
 
-definition entails :: \<open>'m itself \<Rightarrow> ('c, 'v) th \<Rightarrow> ('c, 'v) fm \<Rightarrow> bool\<close> where
-  \<open>entails _ T \<phi> \<longleftrightarrow> (\<forall> \<M> :: ('c, 'v, 'm) interp. is_model_of \<M> T \<longrightarrow> \<M> \<turnstile> \<phi>)\<close>
+lemma is_model_of_conj_iff:
+  \<open>is_model_of \<M> {\<phi> \<^bold>\<and> \<psi>} \<longleftrightarrow>
+    is_model_of \<M> {\<phi>} \<and> is_model_of \<M> {\<psi>}\<close>
+  unfolding is_model_of_def
+proof (intro iffI conjI ballI; (elim conjE)?)
+  fix \<phi>'
+  assume
+    \<open>\<forall> \<phi> \<in> {\<phi> \<^bold>\<and> \<psi>}. \<forall> V. is_vars (dom \<M>) V \<longrightarrow> \<M>,V \<Turnstile> \<phi>\<close> and
+    \<open>\<phi>' \<in> {\<phi>}\<close>
+  then have
+    \<open>\<forall> V. is_vars (dom \<M>) V \<longrightarrow> \<M>,V \<Turnstile> \<phi> \<^bold>\<and> \<psi>\<close> and
+    \<phi>'_is: \<open>\<phi>' = \<phi>\<close>
+    by blast+
+  then have \<open>\<forall> V. is_vars (dom \<M>) V \<longrightarrow> \<M>,V \<Turnstile> \<phi>\<close>
+    by simp 
+  then show \<open>\<forall> V. is_vars (dom \<M>) V \<longrightarrow> \<M>,V \<Turnstile> \<phi>'\<close>
+    unfolding \<phi>'_is . 
+next
+  fix \<psi>'
+  assume
+    \<open>\<forall> \<phi> \<in> {\<phi> \<^bold>\<and> \<psi>}. \<forall> V. is_vars (dom \<M>) V \<longrightarrow> \<M>,V \<Turnstile> \<phi>\<close> and
+    \<open>\<psi>' \<in> {\<psi>}\<close>
+  then have
+    \<open>\<forall> V. is_vars (dom \<M>) V \<longrightarrow> \<M>,V \<Turnstile> \<phi> \<^bold>\<and> \<psi>\<close> and
+    \<psi>'_is: \<open>\<psi>' = \<psi>\<close> 
+    by blast+
+  then have \<open>\<forall> V. is_vars (dom \<M>) V \<longrightarrow> \<M>,V \<Turnstile> \<psi>\<close>
+    by auto 
+  then show \<open>\<forall> V. is_vars (dom \<M>) V \<longrightarrow> \<M>,V \<Turnstile> \<psi>'\<close>
+    unfolding \<psi>'_is .
+next
+  fix \<phi>'
+  assume
+    \<open>\<phi>' \<in> {\<phi> \<^bold>\<and> \<psi>}\<close> and
+    \<open>\<forall> \<phi> \<in> {\<phi>}. \<forall> V. is_vars (dom \<M>) V \<longrightarrow> \<M>,V \<Turnstile> \<phi>\<close> and
+    \<open>\<forall> \<psi> \<in> {\<psi>}. \<forall> V. is_vars (dom \<M>) V \<longrightarrow> \<M>,V \<Turnstile> \<psi>\<close>
+  then have
+    \<phi>'_is: \<open>\<phi>' = \<phi> \<^bold>\<and> \<psi>\<close> and
+    \<open>\<forall> V. is_vars (dom \<M>) V \<longrightarrow> \<M>,V \<Turnstile> \<phi>\<close> and
+    \<open>\<forall> V. is_vars (dom \<M>) V \<longrightarrow> \<M>,V \<Turnstile> \<psi>\<close>
+    by blast+
+  then have \<open>\<forall> V. is_vars (dom \<M>) V \<longrightarrow> \<M>,V \<Turnstile> \<phi> \<^bold>\<and> \<psi>\<close>
+    by simp 
+  then show \<open>\<forall> V. is_vars (dom \<M>) V \<longrightarrow> \<M>,V \<Turnstile> \<phi>'\<close>
+    unfolding \<phi>'_is . 
+qed
+
+definition entails :: \<open>'m itself \<Rightarrow> ('f, 'p, 'v) fm set \<Rightarrow> ('f, 'p, 'v) fm \<Rightarrow> bool\<close> where
+  \<open>entails _ T \<phi> \<longleftrightarrow>
+    (\<forall> \<M> :: ('f, 'p, 'm) model. is_model_of \<M> T \<longrightarrow> (\<forall> V. is_vars (dom \<M>) V \<longrightarrow> \<M>,V \<Turnstile> \<phi>))\<close>
+
+abbreviation entails_set :: \<open>'m itself \<Rightarrow> ('f, 'p, 'v) fm set \<Rightarrow> ('f, 'p, 'v) fm set \<Rightarrow> bool\<close> where
+  \<open>entails_set (m :: 'm itself) M N \<equiv> (\<forall> \<phi> \<in> N. entails m M \<phi>)\<close>
+
+abbreviation entails_\<G> :: \<open>'m itself \<Rightarrow> ('f, 'p, 'v) fm set \<Rightarrow> ('f, 'p, 'v) fm \<Rightarrow> bool\<close> where
+  \<open>entails_\<G> m T \<phi> \<equiv> entails_set m (\<G> T) (\<G> {\<phi>})\<close>
+
+abbreviation entails_\<G>_set :: \<open>'m itself \<Rightarrow> ('f, 'p, 'v) fm set \<Rightarrow> ('f, 'p, 'v) fm set \<Rightarrow> bool\<close> where
+  \<open>entails_\<G>_set m M N \<equiv> entails_set m (\<G> M) (\<G> N)\<close>
 
 syntax
-  "_Entails" :: \<open>('c, 'v) th \<Rightarrow> 'm itself \<Rightarrow> ('c, 'v) fm \<Rightarrow> bool\<close> (\<open>_/ \<Turnstile>\<^sub>_/ _\<close> [80, 20, 80] 80)
-
+  "_Entails" :: \<open>('f, 'p, 'v) fm set \<Rightarrow> 'm itself \<Rightarrow> ('f, 'p, 'v) fm \<Rightarrow> bool\<close>
+    (\<open>_/ \<Turnstile>\<^sub>_/ _\<close> [80, 20, 80] 80)
+  "_Entails_set" :: \<open>('f, 'p, 'v) fm set \<Rightarrow> 'm itself \<Rightarrow> ('f, 'p, 'v) fm set \<Rightarrow> bool\<close>
+    (\<open>_/ \<Turnstile>\<^sup>s\<^sup>e\<^sup>t\<^sub>_/ _\<close> [80, 20, 80] 80)
+  "_Entails_G" :: \<open>'m itself \<Rightarrow> ('f, 'p, 'v) fm set \<Rightarrow> ('f, 'p, 'v) fm \<Rightarrow> bool\<close>
+    (\<open>_/ \<Turnstile>\<^sub>\<G>\<^sub>_/ _\<close> [80, 20, 80] 80)
+  "_Entails_G_set" :: \<open>'m itself \<Rightarrow> ('f, 'p, 'v) fm set \<Rightarrow> ('f, 'p, 'v) fm set \<Rightarrow> bool\<close>
+    (\<open>_/ \<Turnstile>\<^sup>s\<^sup>e\<^sup>t\<^sub>\<G>\<^sub>_/ _\<close> [80, 20, 80] 80)
+  
 translations
-  "T \<Turnstile>\<^sub>M \<phi>" \<rightleftharpoons> "CONST entails T M \<phi>"
+  "T \<Turnstile>\<^sub>m \<phi>" \<rightleftharpoons> "CONST entails m T \<phi>"
+  "M \<Turnstile>\<^sup>s\<^sup>e\<^sup>t\<^sub>m N" \<rightleftharpoons> "CONST entails_set m M N"
+  "T \<Turnstile>\<^sub>\<G>\<^sub>m \<phi>" \<rightleftharpoons> "CONST entails_\<G> m T \<phi>"
+  "M \<Turnstile>\<^sup>s\<^sup>e\<^sup>t\<^sub>\<G>\<^sub>m N" \<rightleftharpoons> "CONST entails_\<G>_set m M N"
 
-abbreviation sat :: \<open>'m itself \<Rightarrow> ('c, 'v) th \<Rightarrow> bool\<close> where
-  \<open>sat _ T \<equiv> (\<exists> \<M> :: ('c, 'v, 'm) interp. is_model_of \<M> T)\<close>
+abbreviation satisfiable :: \<open>('f, 'p, 'v) fm set \<Rightarrow> bool\<close> where
+  \<open>satisfiable T \<equiv>
+    (\<exists> \<M> :: ('f, 'p, ('f, 'v) tm) model. is_canonical \<M> (language T) \<and> is_model_of \<M> T)\<close> 
 
-abbreviation unsat :: \<open>'m itself \<Rightarrow> ('c, 'v) th \<Rightarrow> bool\<close> where
-  \<open>unsat M T \<equiv> \<not> sat M T\<close> 
-
+abbreviation unsatisfiable :: \<open>('f, 'p, 'v) fm set \<Rightarrow> bool\<close> where
+  \<open>unsatisfiable T \<equiv> \<not> satisfiable T\<close>  
+   
 lemma unsat_equiv_no_model:
-  \<open>unsat (_ :: 'm itself) T \<longleftrightarrow> (\<forall> \<M> :: ('c, 'v, 'm) interp. \<not> is_model_of \<M> T)\<close>
-  by (fact not_ex) 
+  \<open>unsatisfiable T \<longleftrightarrow>
+    (\<forall> \<M> :: ('f, 'p, ('f, 'v) tm) model. is_canonical \<M> (language T) \<longrightarrow> \<not> is_model_of \<M> T)\<close>
+  for T :: \<open>('f, 'p, 'v) fm set\<close>
+  by blast 
 
 lemma is_model_of_mono: \<open>T' \<subseteq> T \<Longrightarrow> is_model_of \<M> T \<Longrightarrow> is_model_of \<M> T'\<close>
-  by (simp add: in_mono is_model_of_def) 
+  by (simp add: in_mono is_model_of_def)
 
-(* Theorem 1.6 *)
-theorem sat_compactness: \<open>sat m T \<Longrightarrow> \<forall> T' \<subseteq> T. sat m T'\<close>
-  using is_model_of_mono
-  by blast
+lemma unsat_iff_entails_bot: \<open>T \<Turnstile>\<^sub>m \<^bold>\<bottom> \<longleftrightarrow> (\<forall> \<M> :: ('f, 'p, 'm) model. \<not> is_model_of \<M> T)\<close>
+  for m :: \<open>'m itself\<close>
+proof -
+  have \<open>\<not> (\<M>,\<beta> \<Turnstile> \<^bold>\<bottom>)\<close> for \<M> \<beta>
+    by auto
+  moreover have \<open>\<exists> \<beta>. is_vars (dom \<M>) \<beta>\<close> for \<M>
+    unfolding is_vars_def
+    using model_is_struct struct.M_nonempty
+    by fastforce
+  ultimately have \<open>\<not> (\<forall> \<beta>. is_vars (dom \<M>) \<beta> \<longrightarrow> \<M>,\<beta> \<Turnstile> \<^bold>\<bottom>)\<close> (is \<open>\<not> (?P \<M>)\<close>)
+    for \<M> :: \<open>('f, 'p, 'm) model\<close>
+    by blast 
+  then have \<open>(is_model_of \<M> T \<longrightarrow> ?P m \<M>) \<longleftrightarrow> \<not> is_model_of \<M> T\<close>
+    for \<M> :: \<open>('f, 'p, 'm) model\<close>
+    by blast
+  then have \<open>\<forall> \<M> :: ('f, 'p, 'm) model. (is_model_of \<M> T \<longrightarrow> ?P m \<M>) \<longleftrightarrow> \<not> is_model_of \<M> T\<close>
+    by blast 
+  then have
+    \<open>(\<forall> \<M> :: ('f, 'p, 'm) model. is_model_of \<M> T \<longrightarrow> ?P m \<M>) \<longleftrightarrow>
+     (\<forall> \<M> :: ('f, 'p, 'm) model. \<not> is_model_of \<M> T)\<close>
+    by auto 
+  then show ?thesis 
+    unfolding entails_def
+    by auto
+qed
+
+lemma sat_iff_not_entails_bot: \<open>\<not> T \<Turnstile>\<^sub>m \<^bold>\<bottom> \<longleftrightarrow> (\<exists> \<M> :: ('f, 'p, 'm) model. is_model_of \<M> T)\<close>
+  for m :: \<open>'m itself\<close>
+  by (simp add: unsat_iff_entails_bot) 
+
+subsection \<open>Important results on satisfiability\<close>
+
+lemma map_map_is_map: \<open>map (\<lambda> f. h f x) (map (\<lambda> y. g y) L) = map (\<lambda> y. h (g y) x) L\<close>
+  by simp 
+
+lemma map_map_is_map2: \<open>map (\<lambda> f. f i) (map (\<lambda> x. g x) L) = map (\<lambda> x. g x i) L\<close>
+  by auto
+
+subsubsection \<open>The substitution lemma\<close>
+
+abbreviation (input) \<open>eval_subst \<M> \<beta> \<sigma> v \<equiv> \<lbrakk>\<sigma> v\<rbrakk>\<^bsup>\<M>,\<beta>\<^esup>\<close>
+
+lemma subst_lemma_terms: \<open>\<lbrakk>t \<cdot> \<sigma>\<rbrakk>\<^bsup>\<M>,\<beta>\<^esup> = \<lbrakk>t\<rbrakk>\<^bsup>\<M>,eval_subst \<M> \<beta> \<sigma>\<^esup>\<close>
+proof (induction t)
+  case (Var v)
+  then show ?case
+    by auto 
+next
+  case (Fun f ts)
+
+  have \<open>\<lbrakk>Fun f ts \<cdot> \<sigma>\<rbrakk>\<^bsup>\<M>,\<beta>\<^esup> = \<lbrakk>Fun f [t \<cdot> \<sigma>. t \<leftarrow> ts]\<rbrakk>\<^bsup>\<M>,\<beta>\<^esup>\<close>
+    by auto
+  also have \<open>... = interp_fn \<M> f [\<lbrakk>t\<rbrakk>\<^bsup>\<M>,\<beta>\<^esup>. t \<leftarrow> [t \<cdot> \<sigma>. t \<leftarrow> ts]]\<close>
+    by auto 
+  also have \<open>... = interp_fn \<M> f [\<lbrakk>t \<cdot> \<sigma>\<rbrakk>\<^bsup>\<M>,\<beta>\<^esup>. t \<leftarrow> ts]\<close>
+    unfolding map_map
+    by (meson comp_apply)
+  also have \<open>... = interp_fn \<M> f [\<lbrakk>t\<rbrakk>\<^bsup>\<M>,eval_subst \<M> \<beta> \<sigma>\<^esup>. t \<leftarrow> ts]\<close>
+    using Fun.IH
+    by (smt (verit, best) map_eq_conv) 
+  also have \<open>... = \<lbrakk>Fun f ts\<rbrakk>\<^bsup>\<M>,eval_subst \<M> \<beta> \<sigma>\<^esup>\<close>
+    by auto 
+  finally show ?case .
+qed
+
+lemma eval_indep_\<beta>_if:
+  assumes \<open>\<forall> v \<in> FV_tm t. \<beta> v = \<beta>' v\<close>
+  shows \<open>\<lbrakk>t\<rbrakk>\<^bsup>\<M>,\<beta>\<^esup> = \<lbrakk>t\<rbrakk>\<^bsup>\<M>,\<beta>'\<^esup>\<close>
+    using assms
+proof (induction t)
+  case (Var v)
+  then show ?case
+    by auto 
+next
+  case (Fun f ts)
+  then show ?case
+    by (smt (verit, ccfv_SIG) eval.simps(2) map_eq_conv term.set_intros(4)) 
+qed
+
+lemma eval_fun_upd_if:
+  assumes
+    \<open>v \<in> FV_fm \<phi>\<close> and
+    \<open>v \<noteq> x \<longrightarrow> z \<notin> FV_tm (\<sigma> v)\<close>
+  shows ‹eval_subst \<M> (\<beta>(z := a)) (\<sigma>(x := Var z)) v = ((eval_subst \<M> \<beta> \<sigma>)(x := a)) v\<close>
+proof (cases \<open>v = x\<close>) 
+  case True
+  then show ?thesis
+    by simp 
+next
+  case False
+
+  have \<open>z \<notin> FV_tm (\<sigma> v)\<close>
+    using assms(2)[THEN impE, OF False]
+    by argo
+  then have \<open>\<forall> v' \<in> FV_tm (\<sigma> v). (\<beta>(z := a)) v' = \<beta> v'\<close>
+    by fastforce 
+  then have \<open>\<lbrakk>\<sigma> v\<rbrakk>\<^bsup>\<M>,\<beta>(z := a)\<^esup> = \<lbrakk>\<sigma> v\<rbrakk>\<^bsup>\<M>,\<beta>\<^esup>\<close>
+    by (rule eval_indep_\<beta>_if)
+  then show ?thesis
+    by auto 
+qed
+
+lemma free_set_eq_if:
+  assumes \<open>\<forall> v \<in> FV_fm \<phi> - {x}. z \<notin> FV_tm (\<sigma> v)\<close>
+  shows
+    \<open>{z'. \<exists> y \<in> FV_fm \<phi>. z' \<in> FV_tm ((\<sigma>(x := Var z)) y)} - {z} =
+     {z'. \<exists> y \<in> FV_fm \<phi> - {x}. z' \<in> FV_tm (\<sigma> y)}\<close>
+    (is \<open>?lhs = ?rhs\<close>)
+proof (intro subset_antisym subsetI)
+  fix w
+  assume \<open>w \<in> ?lhs\<close>
+  then have w_neq: \<open>w \<noteq> z\<close> and \<open>\<exists> y \<in> FV_fm \<phi>. w \<in> FV_tm ((\<sigma>(x := Var z)) y)\<close>
+    by auto
+  then obtain y where
+    y_free: \<open>y \<in> FV_fm \<phi>\<close> and
+    w_free: \<open>w \<in> FV_tm ((\<sigma>(x := Var z)) y)\<close>
+    by blast
+  then have y_neq: \<open>y \<noteq> x\<close>
+    using w_neq
+    by force
+
+  have \<open>w \<in> FV_tm (\<sigma> y)\<close>
+    using w_free y_neq
+    by auto
+  moreover have \<open>y \<in> FV_fm \<phi> - {x}\<close>
+    using y_free y_neq
+    by blast
+  ultimately have \<open>\<exists> y \<in> FV_fm \<phi> - {x}. w \<in> FV_tm (\<sigma> y)\<close>
+    by blast  
+  then show \<open>w \<in> ?rhs\<close>
+    by blast   
+next
+  fix w 
+  assume \<open>w \<in> ?rhs›
+  then have \<open>\<exists> y \<in> FV_fm \<phi> - {x}. w \<in> FV_tm (\<sigma> y)\<close>
+    by blast 
+  then obtain y where
+    \<open>y \<in> FV_fm \<phi> - {x}\<close> and
+    w_free: \<open>w \<in> FV_tm (\<sigma> y)\<close>
+    by blast
+  then have y_free: \<open>y \<in> FV_fm \<phi>\<close> and y_neq: \<open>y \<noteq> x\<close>
+    by auto
+  then have w_free': \<open>w \<in> FV_tm ((\<sigma>(x := Var z)) y)\<close>
+    using w_free
+    by force
+
+  have \<open>w \<noteq> z\<close>
+    using y_free y_neq assms w_free
+    by blast
+  moreover have \<open>w \<in> {w. \<exists> y \<in> FV_fm \<phi>. w \<in> FV_tm ((\<sigma>(x := Var z)) y)}\<close>
+    using w_free' y_free
+    by blast
+  ultimately show \<open>w \<in> ?lhs\<close>
+    by blast 
+qed
+
+context
+  assumes UNIV_contains_all_vars: \<open>\<forall> \<phi> :: ('f, 'p, 'v) fm. FV_fm \<phi> \<subset> UNIV\<close>
+begin
+
+lemma free_vars_subst_fm: \<open>FV_fm (\<phi> \<cdot>\<^sub>f\<^sub>m \<sigma>) = {x. \<exists> v \<in> FV_fm \<phi>. x \<in> FV_tm (\<sigma> v)}\<close>
+  for \<phi> :: \<open>('f, 'p, 'v) fm\<close>
+proof (induction rule: subst_fm.induct) 
+  case (1 \<sigma>)
+  then show ?case
+    by auto 
+next
+  case (2 p ts \<sigma>)
+
+  have \<open>FV_fm (Rel p ts \<cdot>\<^sub>f\<^sub>m \<sigma>) = (\<Union> t \<in> set ts. FV_tm (t \<cdot> \<sigma>))\<close>
+    by force 
+  also have \<open>... = (\<Union> t \<in> set ts. \<Union> (FV_tm ` \<sigma> ` FV_tm t))\<close>
+    by (meson vars_term_subst)
+  also have \<open>... = (\<Union> t \<in> set ts. \<Union> v \<in> FV_tm t. FV_tm (\<sigma> v))\<close>
+    by blast
+  also have \<open>... = (\<Union> v \<in> (\<Union> t \<in> set ts. FV_tm t). FV_tm (\<sigma> v))\<close>
+    by blast
+  also have \<open>... = (\<Union> v \<in> FV_fm (Rel p ts). FV_tm (\<sigma> v))\<close>
+    by auto 
+  also have \<open>... = {x. \<exists> v \<in> FV_fm (Rel p ts). x \<in> FV_tm (\<sigma> v)}\<close>
+    by blast 
+  finally show ?case .
+next
+  case (3 \<phi> \<sigma>)
+  then show ?case
+    by auto 
+next
+  case (4 \<phi> \<psi> \<sigma>)
+  then show ?case
+    by auto
+next
+  case ex: (5 x \<phi> \<sigma>)
+
+  show ?case
+  proof (cases \<open>\<exists> y. y \<in> FV_fm (\<^bold>\<exists> x\<^bold>. \<phi>) \<and> x \<in> FV_tm ((\<sigma>(x := Var x)) y)\<close>)
+    case True
+      
+    let ?z = \<open>\<some> z. z \<notin> FV_fm (\<phi> \<cdot>\<^sub>f\<^sub>m \<sigma>(x := Var x))\<close>
+      
+    have z_bound: \<open>\<forall> v \<in> FV_fm \<phi> - {x}. z \<notin> FV_tm (\<sigma> v)\<close>
+      if \<open>z \<notin> FV_fm (\<phi> \<cdot>\<^sub>f\<^sub>m \<sigma>(x := Var x))\<close> 
+      for z
+      by (metis (mono_tags, lifting) DiffD1 DiffD2 True ex.IH(1) fun_upd_other mem_Collect_eq
+          singleton_iff that)
+    moreover obtain z where
+      z_bound': \<open>z \<notin> FV_fm (\<phi> \<cdot>\<^sub>f\<^sub>m \<sigma>(x := Var x))\<close>
+      using ex_fresh_var[OF UNIV_contains_all_vars] .
+    then have \<open>?z \<notin> FV_fm (\<phi> \<cdot>\<^sub>f\<^sub>m \<sigma>(x := Var x))\<close>
+      by (rule someI)
+    ultimately have dummy_z_bound: \<open>\<forall> v \<in> FV_fm \<phi> - {x}. ?z \<notin> FV_tm (\<sigma> v)\<close> . 
+
+    have \<open>FV_fm ((\<^bold>\<exists> x\<^bold>. \<phi>) \<cdot>\<^sub>f\<^sub>m \<sigma>) = (let z = ?z in FV_fm (\<^bold>\<exists> z\<^bold>. (\<phi> \<cdot>\<^sub>f\<^sub>m \<sigma>(x := Var z))))\<close>
+      using True
+      by (smt (verit, ccfv_SIG) Eps_cong subst_fm.simps(5))
+    also have \<open>... = (let z = ?z in FV_fm (\<phi> \<cdot>\<^sub>f\<^sub>m \<sigma>(x := Var z)) - {z})\<close>
+      by auto 
+    also have \<open>... = (let z = ?z in {w. \<exists> v \<in> FV_fm \<phi>. w \<in> FV_tm ((\<sigma>(x := Var z)) v)} - {z})\<close>
+      using True ex.IH(2)
+      by presburger
+    also have \<open>... = {w. \<exists> v \<in> FV_fm \<phi> - {x}. w \<in> FV_tm (\<sigma> v)}\<close>
+      using free_set_eq_if[OF dummy_z_bound]
+      by presburger 
+    also have \<open>... = {w. \<exists> v \<in> FV_fm (\<^bold>\<exists> x\<^bold>. \<phi>). w \<in> FV_tm (\<sigma> v)}\<close>
+      by auto 
+    finally show ?thesis . 
+  next
+    case False
+    then have \<open>\<forall> v \<in> FV_fm (\<^bold>\<exists> x\<^bold>. \<phi>). x \<notin> FV_tm ((\<sigma>(x := Var x)) v)\<close>
+      by blast 
+    then have x_bound: \<open>\<forall> v \<in> FV_fm \<phi> - {x}. x \<notin> FV_tm (\<sigma> v)\<close>
+      by auto 
+
+    have \<open>FV_fm ((\<^bold>\<exists> x\<^bold>. \<phi>) \<cdot>\<^sub>f\<^sub>m \<sigma>) = FV_fm (\<^bold>\<exists> x\<^bold>. (\<phi> \<cdot>\<^sub>f\<^sub>m \<sigma>(x := Var x)))\<close>
+      using False
+      by auto 
+    also have \<open>... = FV_fm (\<phi> \<cdot>\<^sub>f\<^sub>m \<sigma>(x := Var x)) - {x}\<close>
+      by simp 
+    also have \<open>... = {z. \<exists> y \<in> FV_fm \<phi>. z \<in> FV_tm ((\<sigma>(x := Var x)) y)} - {x}\<close>
+      using ex.IH False
+      by presburger 
+    also have \<open>... = {z. \<exists> y \<in> FV_fm \<phi> - {x}. z \<in> FV_tm (\<sigma> y)}\<close>
+      using free_set_eq_if[OF x_bound] .
+    also have \<open>... = {z. \<exists> y \<in> FV_fm (\<^bold>\<exists> x\<^bold>. \<phi>). z \<in> FV_tm (\<sigma> y)}\<close>
+      by simp 
+    finally show ?thesis .
+  qed
+qed
+
+lemma subst_lemma_form: \<open>\<M>,\<beta> \<Turnstile> (\<phi> \<cdot>\<^sub>f\<^sub>m \<sigma>) \<longleftrightarrow> \<M>,(eval_subst \<M> \<beta> \<sigma>) \<Turnstile> \<phi>\<close>
+  for \<phi> :: \<open>('f, 'p, 'v) fm\<close>
+proof (induction \<phi> arbitrary: \<sigma> \<beta>)
+  case (Rel p ts)
+
+  have \<open>\<M>,\<beta> \<Turnstile> (Rel p ts \<cdot>\<^sub>f\<^sub>m \<sigma>) \<longleftrightarrow> \<M>,\<beta> \<Turnstile> Rel p [t \<cdot> \<sigma>. t \<leftarrow> ts]\<close>
+    by auto 
+  also have \<open>... \<longleftrightarrow> [\<lbrakk>t\<rbrakk>\<^bsup>\<M>,\<beta>\<^esup>. t \<leftarrow> [t \<cdot> \<sigma>. t \<leftarrow> ts]] \<in> interp_rel \<M> p\<close>
+    by auto 
+  also have \<open>... \<longleftrightarrow> [\<lbrakk>t \<cdot> \<sigma>\<rbrakk>\<^bsup>\<M>,\<beta>\<^esup>. t \<leftarrow> ts] \<in> interp_rel \<M> p\<close>
+    unfolding map_map
+    by (smt (verit, ccfv_SIG) comp_apply map_eq_conv)  
+  also have \<open>... \<longleftrightarrow> [\<lbrakk>t\<rbrakk>\<^bsup>\<M>,eval_subst \<M> \<beta> \<sigma>\<^esup>. t \<leftarrow> ts] \<in> interp_rel \<M> p\<close>
+    by (simp add: subst_lemma_terms) 
+  also have \<open>... \<longleftrightarrow> \<M>,eval_subst \<M> \<beta> \<sigma> \<Turnstile> Rel p ts\<close>
+    by auto 
+  finally show ?case . 
+next
+  case (Negation \<phi>)
+  then show ?case
+    by auto 
+next
+  case (Conjunction \<phi> \<psi>)
+  then show ?case
+    by auto 
+next
+  case (Existential x \<phi>)
+
+  show ?case
+  proof (cases \<open>\<exists> y. y \<in> FV_fm (\<^bold>\<exists> x\<^bold>. \<phi>) \<and> x \<in> FV_tm ((\<sigma>(x := Var x)) y)\<close>)
+    case True
+
+    have \<open>z \<notin> FV_fm (\<phi> \<cdot>\<^sub>f\<^sub>m \<sigma>(x := Var x)) \<longleftrightarrow> (\<forall> v \<in> FV_fm \<phi>. z \<notin> FV_tm ((\<sigma>(x := Var x)) v))\<close>
+      for z
+      using free_vars_subst_fm
+      by fastforce 
+    also have \<open>... z \<longleftrightarrow> (\<forall> v \<in> FV_fm \<phi>. v \<noteq> x \<longrightarrow> z \<notin> FV_tm (\<sigma> v))\<close>
+      for z
+      using True
+      by force
+    finally have
+      z_not_free_iff: \<open>z \<notin> FV_fm (\<phi> \<cdot>\<^sub>f\<^sub>m \<sigma>(x := Var x)) \<longleftrightarrow> (\<forall> v \<in> FV_fm \<phi>. v \<noteq> x \<longrightarrow> z \<notin> FV_tm (\<sigma> v))\<close>
+      for z .
+
+    let ?z = \<open>\<some> z. z \<notin> FV_fm (\<phi> \<cdot>\<^sub>f\<^sub>m \<sigma>(x := Var x))\<close> 
+
+    have \<open>\<M>,\<beta> \<Turnstile> ((\<^bold>\<exists> x\<^bold>. \<phi>) \<cdot>\<^sub>f\<^sub>m \<sigma>) \<longleftrightarrow> (let z = ?z in \<M>,\<beta> \<Turnstile> (\<^bold>\<exists> z\<^bold>. (\<phi> \<cdot>\<^sub>f\<^sub>m \<sigma>(x := Var z))))\<close>
+      using True
+      by (smt (verit, best) Eps_cong subst_fm.simps(5))  
+    also have \<open>... \<longleftrightarrow> (let z = ?z in \<exists> a \<in> dom \<M>. \<M>,\<beta>(z := a) \<Turnstile> (\<phi> \<cdot>\<^sub>f\<^sub>m \<sigma>(x := Var z)))\<close>
+      by simp
+    also have \<open>... \<longleftrightarrow> (let z = ?z in \<exists> a \<in> dom \<M>. \<M>,eval_subst \<M> (\<beta>(z := a)) (\<sigma>(x := Var z)) \<Turnstile> \<phi>)\<close>
+      using Existential.IH
+      by fastforce 
+    also have \<open>... \<longleftrightarrow> (\<exists> a \<in> dom \<M>. \<M>,(eval_subst \<M> \<beta> \<sigma>)(x := a) \<Turnstile> \<phi>)\<close>
+      (is \<open>?lhs \<longleftrightarrow> ?rhs\<close>)
+    proof (intro iffI)
+      assume ?lhs
+      then obtain a z where
+        a_in_dom: \<open>a \<in> dom \<M>\<close> and
+        z_is: \<open>z = ?z\<close> and 
+        \<phi>_sat: \<open>\<M>,eval_subst \<M> (\<beta>(z := a)) (\<sigma>(x := Var z)) \<Turnstile> \<phi>\<close>
+        by metis
+
+      have \<open>z \<notin> FV_fm (\<phi> \<cdot>\<^sub>f\<^sub>m \<sigma>(x := Var x))\<close>
+        using z_is ex_fresh_var[OF UNIV_contains_all_vars]
+        by (metis someI_ex)
+      then have \<open>\<forall> v \<in> FV_fm \<phi>. v \<noteq> x \<longrightarrow> z \<notin> FV_tm (\<sigma> v)\<close>
+        unfolding z_not_free_iff . 
+      then have
+        \<open>\<forall> v \<in> FV_fm \<phi>. eval_subst \<M> (\<beta>(z := a)) (\<sigma>(x := Var z)) v = ((eval_subst \<M> \<beta> \<sigma>)(x := a)) v\<close>
+        by (metis eval_fun_upd_if) 
+      then show ?rhs
+        using \<phi>_sat a_in_dom
+        by (smt (verit, best) satisfies_indep_\<beta>_if) 
+    next
+      assume ?rhs
+      then obtain a where
+        a_in_dom: \<open>a \<in> dom \<M>\<close> and
+        \<phi>_sat: \<open>\<M>,(eval_subst \<M> \<beta> \<sigma>)(x := a) \<Turnstile> \<phi>\<close>
+        by blast
+
+      obtain z where
+        \<open>z \<notin> FV_fm (\<phi> \<cdot>\<^sub>f\<^sub>m \<sigma>(x := Var x))\<close>
+        using ex_fresh_var[OF UNIV_contains_all_vars] . 
+      then have \<open>?z \<notin> FV_fm (\<phi> \<cdot>\<^sub>f\<^sub>m \<sigma>(x := Var x))\<close>
+        by (metis someI_ex) 
+      then have \<open>\<forall> v \<in> FV_fm \<phi>. v \<noteq> x \<longrightarrow> ?z \<notin> FV_tm (\<sigma> v)\<close>
+        unfolding z_not_free_iff . 
+      then have
+        \<open>let z = ?z in \<forall> v \<in> FV_fm \<phi>. eval_subst \<M> (\<beta>(z := a)) (\<sigma>(x := Var z)) v =
+         ((eval_subst \<M> \<beta> \<sigma>)(x := a)) v\<close>
+        by (metis eval_fun_upd_if)
+      then show ?lhs
+        by (smt (verit, ccfv_threshold) \<phi>_sat a_in_dom satisfies_indep_\<beta>_if) 
+    qed
+    also have \<open>... \<longleftrightarrow> \<M>,eval_subst \<M> \<beta> \<sigma> \<Turnstile> (\<^bold>\<exists> x\<^bold>. \<phi>)\<close>
+      by simp 
+    finally show ?thesis .
+  next
+    case False
+
+    have \<open>\<forall> v \<in> FV_fm \<phi>. v \<noteq> x \<longrightarrow> v \<in> FV_fm (\<^bold>\<exists> x\<^bold>. \<phi>)\<close>
+      by auto  
+    then have \<open>\<forall> v \<in> FV_fm \<phi>. v \<noteq> x \<longrightarrow> x \<notin> FV_tm ((\<sigma>(x := Var x)) v)\<close>
+      using False
+      by blast 
+    then have x_bound: \<open>\<forall> v \<in> FV_fm \<phi>. v \<noteq> x \<longrightarrow> x \<notin> FV_tm (\<sigma> v)\<close>
+      by fastforce 
+
+    have \<open>\<M>,\<beta> \<Turnstile> ((\<^bold>\<exists> x\<^bold>. \<phi>) \<cdot>\<^sub>f\<^sub>m \<sigma>) \<longleftrightarrow> \<M>,\<beta> \<Turnstile> (\<^bold>\<exists> x\<^bold>. (\<phi> \<cdot>\<^sub>f\<^sub>m \<sigma>(x := Var x)))\<close>
+      using False
+      by auto 
+    also have \<open>... \<longleftrightarrow> (\<exists> a \<in> dom \<M>. \<M>,\<beta>(x := a) \<Turnstile> (\<phi> \<cdot>\<^sub>f\<^sub>m \<sigma>(x := Var x)))\<close>
+      by auto 
+    also have \<open>... \<longleftrightarrow> (\<exists> a \<in> dom \<M>. \<M>,eval_subst \<M> (\<beta>(x := a)) (\<sigma>(x := Var x)) \<Turnstile> \<phi>)\<close>
+      using Existential.IH
+      by blast 
+    also have \<open>... \<longleftrightarrow> (\<exists> a \<in> dom \<M>. \<M>,(eval_subst \<M> \<beta> \<sigma>)(x := a) \<Turnstile> \<phi>)\<close>
+      by (smt (verit, ccfv_SIG) eval_fun_upd_if fun_upd_def satisfies_indep_\<beta>_if x_bound) 
+    also have \<open>... \<longleftrightarrow> \<M>,eval_subst \<M> \<beta> \<sigma> \<Turnstile> (\<^bold>\<exists> x\<^bold>. \<phi>)\<close>
+      by auto 
+    finally show ?thesis .
+  qed
+next
+  case Bot
+  then show ?case
+    by auto  
+qed
+
+lemma eval_in_dom_if: \<open>is_vars (dom \<M>) \<beta> \<Longrightarrow> \<lbrakk>t\<rbrakk>\<^bsup>\<M>,\<beta>\<^esup> \<in> dom \<M>\<close>
+proof (induction t)   
+  case (Fun f ts)
+
+  have \<open>\<lbrakk>Fun f ts\<rbrakk>\<^bsup>\<M>,\<beta>\<^esup> = interp_fn \<M> f [\<lbrakk>t\<rbrakk>\<^bsup>\<M>,\<beta>\<^esup>. t \<leftarrow> ts]\<close>
+    by auto 
+  moreover have \<open>\<forall> t \<in> set ts. \<lbrakk>t\<rbrakk>\<^bsup>\<M>,\<beta>\<^esup> \<in> dom \<M>\<close>
+    using Fun.IH Fun.prems
+    by blast 
+  then have \<open>interp_fn \<M> f [\<lbrakk>t\<rbrakk>\<^bsup>\<M>,\<beta>\<^esup>. t \<leftarrow> ts] \<in> dom \<M>\<close>
+    by (simp add: FN_dom_to_dom) 
+  ultimately show ?case
+    by argo 
+qed auto
+
+lemma model_is_model_of_all_subst: \<open>is_model_of \<M> {\<phi>} \<Longrightarrow> \<forall> \<sigma>. is_model_of \<M> {\<phi> \<cdot>\<^sub>f\<^sub>m \<sigma>}\<close>
+  for
+    \<phi> :: \<open>('f, 'p, 'v) fm\<close> and
+    \<M> :: \<open>('f, 'p, 'm) model\<close>
+  unfolding is_model_of_def
+proof (intro allI ballI impI) 
+  fix \<sigma> \<phi>' and \<beta> :: \<open>'v \<Rightarrow> 'm\<close> 
+  assume
+    \<phi>_sat: \<open>\<forall> \<phi> \<in> {\<phi>}. \<forall> \<beta>. is_vars (dom \<M>) \<beta> \<longrightarrow> \<M>,\<beta> \<Turnstile> \<phi>\<close> and
+    \<phi>'_in: \<open>\<phi>' \<in> {\<phi> \<cdot>\<^sub>f\<^sub>m \<sigma>}\<close> and
+    \<beta>_val: \<open>is_vars (dom \<M>) \<beta>\<close>
+
+  have \<open>\<phi>' = \<phi> \<cdot>\<^sub>f\<^sub>m \<sigma>\<close>
+    using \<phi>'_in
+    by blast  
+  moreover have \<open>\<M>,\<beta> \<Turnstile> (\<phi> \<cdot>\<^sub>f\<^sub>m \<sigma>) \<longleftrightarrow> \<M>,eval_subst \<M> \<beta> \<sigma> \<Turnstile> \<phi>\<close>
+    by (simp add: subst_lemma_form)
+  moreover have \<open>is_vars (dom \<M>) (eval_subst \<M> \<beta> \<sigma>)\<close>
+    unfolding is_vars_def
+    using eval_in_dom_if[OF \<beta>_val]
+    by blast 
+  then have \<open>\<M>,eval_subst \<M> \<beta> \<sigma> \<Turnstile> \<phi>\<close>
+    using \<phi>_sat
+    by blast 
+  ultimately show \<open>\<M>,\<beta> \<Turnstile> \<phi>'\<close>
+    by blast 
+qed
+
+lemma is_model_of_iff: \<open>is_model_of \<M> T \<longleftrightarrow> (\<forall> \<phi> \<in> T. is_model_of \<M> {\<phi>})\<close>
+  unfolding is_model_of_def
+  by blast 
+
+lemma is_model_of_indiv: \<open>is_model_of \<M> T \<Longrightarrow> \<forall> \<sigma>. \<forall> \<phi> \<in> T. is_model_of \<M> {\<phi> \<cdot>\<^sub>f\<^sub>m \<sigma>}\<close>
+  for
+    T :: \<open>('f, 'p, 'v) fm set\<close> and
+    \<M> :: \<open>('f, 'p, 'm) model\<close>
+  by (meson is_model_of_iff model_is_model_of_all_subst)
+
+lemma is_model_of_grounding: \<open>is_model_of \<M> T \<Longrightarrow> is_model_of \<M> (\<G> T)\<close>
+  for
+    T :: \<open>('f, 'p, 'v) fm set\<close> and
+    \<M> :: \<open>('f, 'p, 'm) model\<close>
+  using is_model_of_iff is_model_of_indiv
+  by fastforce
+
+subsubsection \<open>Grounding equi-satisfiability\<close>
+
+lemma grounding_bot_is_bot[simp]: \<open>\<G> {\<^bold>\<bottom>} = {\<^bold>\<bottom>}\<close>
+  using ex_ground_subst
+  by auto
+
+lemma \<open>\<not> N \<Turnstile>\<^sub>m \<^bold>\<bottom> \<longleftrightarrow> \<not> N \<Turnstile>\<^sub>\<G>\<^sub>m \<^bold>\<bottom>\<close>
+  for
+    N :: \<open>('f, 'p, 'v) fm set\<close> and
+    m :: \<open>'m itself\<close>
+proof (intro iffI)
+  assume \<open>\<not> N \<Turnstile>\<^sub>m \<^bold>\<bottom>\<close>
+  then have \<open>\<exists> \<M> :: ('f, 'p, 'm) model. is_model_of \<M> N\<close>
+    using unsat_iff_entails_bot
+    by blast
+  then have \<open>\<exists> \<M> :: ('f, 'p, 'm) model. is_model_of \<M> (\<G> N)\<close>
+    using is_model_of_grounding
+    by blast
+  then show \<open>\<not> N \<Turnstile>\<^sub>\<G>\<^sub>m \<^bold>\<bottom>\<close>
+    using grounding_bot_is_bot unsat_iff_entails_bot
+    by auto
+next
+  assume \<open>\<not> N \<Turnstile>\<^sub>\<G>\<^sub>m \<^bold>\<bottom>\<close>
+  show \<open>\<not> N \<Turnstile>\<^sub>m \<^bold>\<bottom>\<close>
+    (* TODO *)
+    sorry 
+qed
+
+end (* context *)
+
+subsubsection \<open>Other results\<close>
+
+lemma satD:
+  \<open>satisfiable T \<Longrightarrow>
+    \<exists> \<M> :: ('f, 'p, ('f, 'v) tm) model. is_canonical \<M> (language T) \<and> is_model_of \<M> T\<close>
+  for T :: \<open>('f, 'p, 'v) fm set\<close> .
+
+lemma satI: \<open>\<exists> \<M> :: ('f, 'p, 'm) model. is_model_of \<M> T \<Longrightarrow> satisfiable T\<close>
+  for T :: \<open>('f, 'p, 'v) fm set\<close>
+  sorry 
+
 
 
 section \<open>Filters and ultrafilters\<close> 
@@ -244,15 +1226,41 @@ locale filter =
 (* NOTE: This definition does not correspond to the one of the article.
  * In fact, the one in the article seems to be totally wrong and does not exclude the empty set
  * from being a filter of an empty set.
- * We also cannot prove the lemma 2.2 (counter example: \<open>F = {}\<close> and \<open>S = {}\<close>.
+ * We also cannot prove the lemma 2.2 (counter example: \<open>F = {}\<close> and \<open>S = {}\<close>).
  *
  * Instead, we take the definition from the book:
- * ``Set Theory: The Third Millennium Edition, revised and expanded'' (pp 72-75) *)
+ * ``Set Theory: The Third Millennium Edition, revised and expanded'' (pp 72-75)
+ *
+ * Other variants exists (e.g. without @{thm S_in_F}) but they should be all equivalent. *)
 begin
 
 lemma F_not_empty: \<open>F \<noteq> {}\<close>
   using S_in_F
   by blast
+
+lemma in_F_subset_S: \<open>x \<in> F \<Longrightarrow> x \<subseteq> S\<close>
+  using F_family_of_subsets_of_S
+  by blast 
+
+lemma closed_int': \<open>A \<subseteq> S \<Longrightarrow> B \<subseteq> S \<Longrightarrow> A \<inter> B \<in> F \<Longrightarrow> A \<in> F \<and> B \<in> F\<close>
+proof (intro conjI) 
+  assume
+    A_subset_S: \<open>A \<subseteq> S\<close> and
+    B_subset_S: \<open>B \<subseteq> S\<close> and 
+    inter_in_F: \<open>A \<inter> B \<in> F\<close>
+
+  have \<open>A \<inter> B \<subseteq> A\<close>
+    by blast 
+  then show \<open>A \<in> F\<close>
+    using upwards_closed[OF in_F_subset_S[OF inter_in_F] A_subset_S inter_in_F]
+    by auto 
+
+  have \<open>A \<inter> B \<subseteq> B\<close>
+    by blast
+  then show \<open>B \<in> F\<close>
+    using upwards_closed[OF in_F_subset_S[OF inter_in_F] B_subset_S inter_in_F]
+    by blast 
+qed
 
 text \<open>
   A filter is maximal under inclusion if there does not exists a filter strictly containing it.
@@ -289,7 +1297,7 @@ proof (intro conjI allI impI)
     by fastforce
   show \<open>A \<subseteq> S \<Longrightarrow> B \<subseteq> S \<Longrightarrow> A \<in> \<Inter> \<F> \<Longrightarrow> A \<subseteq> B \<Longrightarrow> B \<in> \<Inter> \<F>\<close>
     (* Slow *)
-    by (smt (verit, best) CollectD FOL_Compactness.filter_def Inter_iff \<F>_family_of_filters) 
+    by (smt (verit, best) CollectD filter_def Inter_iff \<F>_family_of_filters) 
 qed
 
 lemma Union_chain_is_filter:
@@ -312,7 +1320,7 @@ proof (intro conjI allI impI)
     by (metis CollectD Union_iff \<C>_filter_chain \<C>_non_empty filter.S_in_F subset_chain_def
         subset_empty subset_iff)
   show \<open>{} \<notin> \<Union> \<C>\<close>
-    by (metis CollectD FOL_Compactness.filter_def Union_iff \<C>_filter_chain subset_chain_def
+    by (metis CollectD filter_def Union_iff \<C>_filter_chain subset_chain_def
         subset_iff)
   show \<open>A \<in> \<Union> \<C> \<Longrightarrow> B \<in> \<Union> \<C> \<Longrightarrow> A \<inter> B \<in> \<Union> \<C>\<close>
     using \<C>_filter_chain \<C>_non_empty
@@ -332,7 +1340,7 @@ text \<open>
 \<close> 
 
 definition fip :: \<open>'a set set \<Rightarrow> bool\<close> where
-  \<open>fip \<G> \<longleftrightarrow> (\<forall> H \<subseteq> \<G>. finite H \<longrightarrow> \<Inter> H \<noteq> {})\<close>  
+  \<open>fip G \<longleftrightarrow> (\<forall> H \<subseteq> G. finite H \<longrightarrow> \<Inter> H \<noteq> {})\<close>  
 
 lemma trivial_filter: \<open>S \<noteq> {} \<Longrightarrow> filter {S} S\<close>
   unfolding filter_def
@@ -511,8 +1519,8 @@ next
 qed
 
 text \<open>
-  An ultrafilter \<open>F\<close> is a filter \<open>F\<close> for which, for all set \<open>A\<close> of the universe, either \<open>A\<close> or \<open>-A\<close>
-  is in \<open>F\<close>.
+  An ultrafilter \<open>F\<close> on \<open>S\<close> is a filter \<open>F\<close> on \<open>S\<close> for which, for all subset \<open>A\<close> of \<open>S\<close>,
+  either \<open>A\<close> or \<open>S - A\<close> is in \<open>F\<close>.
 \<close> 
 
 locale ultrafilter = filter F S
@@ -566,7 +1574,7 @@ proof (intro iffI conjI; (elim conjE)?)
         then have X_inter_Y_empty: \<open>X \<inter> Y = {}\<close>
           by blast
         then have \<open>X \<subseteq> S - Y\<close>
-          by (metis Diff_partition Diff_subset_conv Diff_triv FOL_Compactness.filter_def F_filter
+          by (metis Diff_partition Diff_subset_conv Diff_triv filter_def F_filter
               PowD X_in_F Y_subset_S subsetD) 
         then have \<open>S - Y \<in> F\<close>
           by (smt (verit, del_insts) Diff_subset F_filter X_in_F dual_order.strict_trans1
@@ -596,7 +1604,8 @@ proof (intro iffI conjI; (elim conjE)?)
         case False
 
         have \<open>\<Inter> (H - {Y}) \<in> F\<close>
-          by (rule Inter_finite_subset_in_filter_if[OF F_filter False H_minus_Y_subset_F finite_H_minus_Y])
+          by (rule Inter_finite_subset_in_filter_if
+                [OF F_filter False H_minus_Y_subset_F finite_H_minus_Y])
         then have \<open>Y \<inter> \<Inter> (H - {Y}) \<noteq> {}\<close>
           using inter_Y_not_empty
           by auto 
@@ -669,7 +1678,7 @@ proof -
     for \<C>
   proof -
     have \<open>filter (\<Union> \<C>) S\<close>
-      by (smt (verit) Union_chain_is_filter mem_Collect_eq subset_chain_def subset_iff that(1) that(2)) 
+      by (smt (verit) Union_chain_is_filter mem_Collect_eq subset_chain_def subset_iff that) 
     then show \<open>\<Union> \<C> \<in> ?P\<close>
       by (metis (no_types, lifting) CollectD CollectI Sup_bot_conv(1) Sup_upper2 filter.F_not_empty
           subsetD subset_chain_def that(1))
@@ -687,47 +1696,1255 @@ proof -
     by blast
 qed   
 
+
+
 section \<open>Ultraproducts\<close> 
 
+locale ultraprod =
+  fixes
+    I :: \<open>'i set\<close> and
+    F :: \<open>'i set set\<close> and
+    \<M> :: \<open>'i \<Rightarrow> ('f, 'p, 'm) model\<close> and 
+    VARs :: \<open>'i \<Rightarrow> 'v \<Rightarrow> 'm\<close>
+  assumes
+    all_structs: \<open>\<forall> i \<in> I. is_vars (dom (\<M> i)) (VARs i)\<close> and
+    F_ultrafilter: \<open>ultrafilter F I\<close>
+begin 
+
+lemma F_filter: \<open>filter F I\<close>
+  by (rule ultrafilter_is_filter[OF F_ultrafilter]) 
+
 text \<open>
-  We go back to model theory. 
+  We go back to model theory.
+
+  First, we define a natural equivalence relation on the indexed cartesian product.
 \<close>
 
-(* definition eq_rel :: \<open>'i set \<Rightarrow> 'i set set \<Rightarrow> ('i \<Rightarrow> 'm) \<Rightarrow> ('i \<Rightarrow> 'm) \<Rightarrow> bool\<close> where
-  \<open>eq_rel I S a b \<longleftrightarrow> { i \<in> I. a i = b i } \<in> S\<close>
+abbreviation prod_eq :: \<open>('i \<Rightarrow> 'm) rel\<close> (\<open>'(\<sim>')\<close>) where
+  \<open>prod_eq \<equiv>
+    { (f, g). f \<in> (\<Pi> i \<in> I. dom (\<M> i)) \<and> g \<in> (\<Pi> i \<in> I. dom (\<M> i)) \<and> {i \<in> I. f i = g i} \<in> F }\<close>
 
-syntax
-  "_Eq" :: \<open>('i \<Rightarrow> 'm) \<Rightarrow> 'i set \<Rightarrow> 'i set set \<Rightarrow> ('i \<Rightarrow> 'm) \<Rightarrow> bool\<close> (\<open>_ \<sim>\<^bsub>_,_\<^esub> _\<close> [50, 40, 40, 50] 50)
+lemma refl_prod_eq: \<open>refl_on (\<Pi> i \<in> I. dom (\<M> i)) (\<sim>)\<close>
+proof
+  show \<open>(\<sim>) \<subseteq> (\<Pi> i \<in> I. dom (\<M> i)) \<times> (\<Pi> i \<in> I. dom (\<M> i))\<close>
+    by blast 
+next 
+  fix f 
+  assume f_in: \<open>f \<in> (\<Pi> i \<in> I. dom (\<M> i))\<close>
+  then show \<open>(f, f) \<in> (\<sim>)\<close>
+  proof -
+    have \<open>{i \<in> I. f i = f i} = I\<close>
+      by auto 
+    moreover have \<open>I \<in> F\<close>
+      using filter.S_in_F[OF F_filter] .
+    ultimately have \<open>{i \<in> I. f i = f i} \<in> F\<close>
+      by presburger 
+    then show ?thesis
+      using f_in
+      by blast 
+  qed
+qed 
 
-translations
-  "a \<sim>\<^bsub>I,S\<^esub> b" \<rightleftharpoons> "CONST eq_rel I S a b"
+lemma sym_prod_eq: \<open>sym (\<sim>)\<close>
+proof
+  fix f g :: \<open>'i \<Rightarrow> 'm\<close>
+  assume f_sim_g: \<open>(f, g) \<in> (\<sim>)\<close>
+  then have \<open>{i \<in> I. f i = g i} \<in> F\<close>
+    by blast 
+  then have \<open>{i \<in> I. g i = f i} \<in> F\<close>
+    by (smt (verit, ccfv_threshold) Collect_cong) 
+  then show \<open>(g, f) \<in> (\<sim>)\<close>
+    using f_sim_g
+    by blast 
+qed
 
-definition eq_class :: \<open>'a \<Rightarrow> ('a \<Rightarrow> 'a \<Rightarrow> bool) \<Rightarrow> 'a set\<close> (\<open>[_]\<^bsub>_\<^esub>\<close>) where
-  \<open>[x]\<^bsub>eq\<^esub> \<equiv> { y. eq x y }\<close> 
+lemma trans_prod_eq: \<open>trans (\<sim>)\<close>
+proof
+  fix f g h
+  assume
+    f_sim_g: \<open>(f, g) \<in> (\<sim>)\<close> and
+    g_sim_h: \<open>(g, h) \<in> (\<sim>)\<close>
+  then have
+    \<open>{i \<in> I. f i = g i} \<in> F\<close> (is \<open>?S1 \<in> _\<close>) and
+    \<open>{i \<in> I. g i = h i} \<in> F\<close> (is \<open>?S2 \<in> _\<close>)
+    by blast+
+  then have \<open>?S1 \<inter> ?S2 \<in> F\<close>
+    using filter.closed_int[OF F_filter]
+    by blast
+  then have \<open>{i \<in> I. f i = g i \<and> g i = h i} \<in> F\<close> (is \<open>?S3 \<in> _\<close>)
+    by (simp add: Collect_conj_eq Int_left_commute inf.commute)
+  moreover have \<open>?S3 \<subseteq> {i \<in> I. f i = h i}\<close>
+    by auto 
+  moreover have \<open>{i \<in> I. f i = h i} \<subseteq> I\<close>
+    by auto 
+  ultimately show \<open>(f, h) \<in> (\<sim>)\<close>
+    using filter.upwards_closed[OF F_filter, of \<open>{i \<in> I. f i = g i \<and> g i = h i}\<close>] f_sim_g g_sim_h
+    by blast   
+qed
 
-definition quotient_set :: \<open>'a set \<Rightarrow> ('a \<Rightarrow> 'a \<Rightarrow> bool) \<Rightarrow> 'a set set\<close> where
-  \<open>quotient_set E eq \<equiv> { [x]\<^bsub>eq\<^esub> | x. x \<in> E }\<close> *) 
+lemma equiv_prod_eq: \<open>equiv (\<Pi> i \<in> I. dom (\<M> i)) (\<sim>)\<close>
+  by (simp add: equivI refl_prod_eq sym_prod_eq trans_prod_eq) 
+
+
+lemma prod_eq_class_nonempty: \<open>f \<in> (\<Pi> i \<in> I. dom (\<M> i)) \<Longrightarrow> prod_eq `` {f} \<noteq> {}\<close>
+  using equiv_class_self equiv_prod_eq
+  by fastforce
+
+text \<open>
+  The ultraproduct of \<open>S\<close> by the ultrafilter \<open>U\<close> is the quotient set of the cartesian product
+  \<open>\<Pi> i \<in> I. S i\<close> by the equivalence relation \<open>prod_eq' I U\<close>.
+\<close> 
+
+(* Definition 2.5 *)
+abbreviation ultraproduct :: \<open>('i \<Rightarrow> 'm set) \<Rightarrow> ('i \<Rightarrow> 'm) set set\<close> where
+  \<open>ultraproduct S \<equiv> (\<Pi> i \<in> I. S i) // (\<sim>)\<close>
+
+lemma ultraproduct_nonempty: \<open>\<forall> i \<in> I. S i \<noteq> {} \<Longrightarrow> ultraproduct S \<noteq> {}\<close>
+  by auto
+
+section \<open>Models, using ultraproducts\<close>
+
+definition rep :: \<open>('i \<Rightarrow> 'm) set \<Rightarrow> 'i \<Rightarrow> 'm\<close> where
+  \<open>rep cls = (\<some> x. x \<in> cls)\<close>
+
+lemma rep_in_cls: \<open>C \<noteq> {} \<Longrightarrow> rep C \<in> C\<close>
+  unfolding rep_def
+  by (simp add: some_in_eq)
+
+lemma rep_relates_to_elem_of_equiv_class:
+  \<open>f \<in> (\<Pi> i \<in> I. dom (\<M> i)) \<Longrightarrow> (rep ((\<sim>) `` {f}), f) \<in> (\<sim>)\<close>
+  unfolding rep_def
+  by (metis (no_types, lifting) Image_singleton_iff equiv_class_self equiv_prod_eq someI_ex sym_def
+      sym_prod_eq) 
+
+lemma rep_of_elem_ultraproduct_in_pi:
+  \<open>x \<in> ultraproduct (dom \<circ> \<M>) \<Longrightarrow> rep x \<in> (\<Pi> i \<in> I. dom (\<M> i))\<close>
+  using equiv_Eps_preserves equiv_prod_eq rep_def
+  by auto
+
+lemma elem_in_pi_to_ultraproduct:
+  \<open>x \<in> (\<Pi> i \<in> I. dom (\<M> i)) \<Longrightarrow> (\<sim>) `` {x} \<in> ultraproduct (dom \<circ> \<M>)\<close>
+  by (metis (no_types, lifting) Pi_iff comp_apply quotientI) 
+
+lemma elem_eq_class_in_pi: \<open>(\<sim>) `` {f} \<in> ultraproduct (dom \<circ> \<M>) \<Longrightarrow> f \<in> (\<Pi> i \<in> I. dom (\<M> i))\<close>
+  by (smt (verit, del_insts) Pi_iff comp_def disjnt_equiv_class equiv_class_eq_iff equiv_prod_eq
+      quotientE) 
+
+lemma struct_Mi: \<open>\<forall> i \<in> I. struct (dom (\<M> i)) (interp_fn (\<M> i)) (interp_rel (\<M> i))\<close>
+  using model_is_struct
+  by blast 
+
+lemma vars_Mi: \<open>\<forall> i \<in> I. is_vars (dom (\<M> i)) (VARs i)\<close>
+  using all_structs
+  by blast
+
+text \<open>
+  The model \<open>\<UU>\<close> on universe \<open>A\<close> is obtained by interpreting the language as follows:
+  \<^item> If \<open>P(x\<^sub>1, \<dots>, x\<^sub>n)\<close> is a predicate, then \<open>P\<^sup>\<UU>([f\<^sub>1], \<dots>, [f\<^sub>n])\<close> iff
+    \<open>{x \<in> I. P\<^bsup>\<UU>\<^sub>x\<^esup>(f\<^sub>1(x), \<dots>, f\<^sub>n(x))} \<in> F\<close>;
+  \<^item> If \<open>F(x\<^sub>1, \<dots>, x\<^sub>n)\<close> is a function, then \<open>F\<^sup>U([f\<^sub>1], \<dots>, [f\<^sub>n]) = [f]\<close> where
+    for all \<open>x \<in> I\<close>, \<open>f(x) = F\<^bsup>\<UU>\<^sub>x\<^esup>(f\<^sub>1(x), \<dots>, f\<^sub>n(x))\<close>.
+\<close>
+
+abbreviation A :: \<open>('i \<Rightarrow> 'm) set set\<close> where
+  \<open>A \<equiv> ultraproduct (dom \<circ> \<M>)\<close>
+
+lemma A_nonempty: \<open>A \<noteq> {}\<close>
+  using struct_Mi struct.M_nonempty
+  by auto 
+
+definition FN :: \<open>'f \<Rightarrow> ('i \<Rightarrow> 'm) set list \<Rightarrow> ('i \<Rightarrow> 'm) set\<close> where
+  \<open>FN f e \<equiv> (\<sim>) `` {\<lambda> i \<in> I. interp_fn (\<M> i) f [rep e\<^sub>i i. e\<^sub>i \<leftarrow> e]}\<close>
+
+definition REL :: \<open>'p \<Rightarrow> ('i \<Rightarrow> 'm) set list set\<close> where
+  \<open>REL p = {e. (\<forall> x \<in> set e. x \<in> A) \<and> {i \<in> I. [rep e\<^sub>i i. e\<^sub>i \<leftarrow> e] \<in> interp_rel (\<M> i) p} \<in> F}\<close> 
+
+sublocale \<A>_struct: struct A FN REL
+  unfolding struct_def 
+proof (intro allI impI conjI ballI)
+  show \<open>A \<noteq> {}\<close>
+    by (fact A_nonempty)
+next
+  fix f es
+  assume \<open>\<forall> e \<in> set es. e \<in> A\<close>
+  then have \<open>\<forall> e \<in> set es. rep e \<in> (\<Pi> i \<in> I. dom (\<M> i))\<close>
+    using A_nonempty rep_of_elem_ultraproduct_in_pi
+    by auto 
+  then have \<open>\<forall> e \<in> set [rep e\<^sub>i. e\<^sub>i \<leftarrow> es]. e \<in> (\<Pi> i \<in> I. dom (\<M> i))\<close>
+    by simp 
+  then have \<open>\<forall> e \<in> set [rep e\<^sub>i. e\<^sub>i \<leftarrow> es]. \<forall> i \<in> I. e i \<in> dom (\<M> i)\<close>
+    by blast
+  then have \<open>\<forall> i \<in> I. \<forall> e \<in> set [rep e\<^sub>i i. e\<^sub>i \<leftarrow> es]. e \<in> dom (\<M> i)\<close>
+    by simp 
+  then have \<open>interp_fn (\<M> i) f [rep e\<^sub>i i. e\<^sub>i \<leftarrow> es] \<in> dom (\<M> i)\<close>
+    if \<open>i \<in> I\<close> 
+    for i
+    using struct.FN_dom_to_dom[OF struct_Mi[rule_format, OF that]] that 
+    by blast
+  then have \<open>(\<lambda> i \<in> I. interp_fn (\<M> i) f [rep e\<^sub>i i. e\<^sub>i \<leftarrow> es]) \<in> (\<Pi> i \<in> I. dom (\<M> i))\<close>
+    by blast 
+  then show \<open>FN f es \<in> A\<close>
+    unfolding FN_def
+    by (smt (verit, best) Pi_mono comp_eq_dest_lhs quotientI subset_iff)
+next
+  fix p es e
+  assume
+    \<open>es \<in> REL p\<close> and
+    e_in: \<open>e \<in> set es\<close>
+  then have \<open>\<forall> e \<in> set es. e \<in> A\<close> and \<open>{i \<in> I. [rep e\<^sub>i i. e\<^sub>i \<leftarrow> es] \<in> interp_rel (\<M> i) p} \<in> F\<close> 
+    unfolding REL_def
+    by blast+  
+  then show \<open>e \<in> A\<close>
+    using e_in
+    by blast
+qed  
+
+abbreviation \<open>\<A> \<equiv> Abs_model (A, FN, REL)\<close> 
+
+lemma dom_\<A> [simp]: \<open>dom \<A> = A\<close>
+  using \<A>_struct.struct_axioms
+  by auto 
+
+lemma interp_fn_\<A> [simp]: \<open>interp_fn \<A> = FN\<close>
+  using \<A>_struct.struct_axioms
+  by auto
+
+lemma interp_rel_\<A> [simp]: \<open>interp_rel \<A> = REL\<close>
+  using \<A>_struct.struct_axioms
+  by auto
+
+text \<open>
+  We show that the choice of representatives in \<open>\<UU>\<close> does not matter. 
+\<close>
+
+lemma list_all2_iff_eq_maps:
+  assumes
+    \<open>length xs = length ys\<close> 
+  shows
+    \<open>list_all2 (\<lambda> x y. f x = g y) xs ys \<longleftrightarrow> [f x. x \<leftarrow> xs] = [g y. y \<leftarrow> ys]\<close>
+  by (induction xs ys rule: list_induct2', auto) 
+
+lemma lists_related_to_inter_in_filter:
+  assumes
+    \<open>as \<noteq> []\<close> and
+    \<open>length as = length bs\<close> and
+    \<open>list_all2 (in_rel (\<sim>)) as bs\<close>
+  shows \<open>\<Inter> (set (map2 (\<lambda> a b. {i \<in> I. a i = b i}) as bs)) \<in> F\<close>
+proof -
+  have \<open>list_all (\<lambda> A. A \<in> F) (map2 (\<lambda> a b. {i \<in> I. a i = b i}) as bs)\<close>
+    using assms(2, 3)
+    by (auto simp add: list_all2_conv_all_nth list_all_length)
+  then show \<open>\<Inter> (set (map2 (\<lambda> a b. {i \<in> I. a i = b i}) as bs)) \<in> F\<close>
+    using assms(2, 3)
+  proof (induction arbitrary: bs rule: list_nonempty_induct[OF assms(1)])
+    case (1 x)
+    then obtain y where
+      \<open>bs = [y]\<close> and
+      \<open>(x, y) \<in> (\<sim>)\<close>
+      by (metis (no_types, lifting) in_rel_def list_all2_Cons1 list_all2_Nil) 
+    then have
+      \<open>map2 (\<lambda> a b. {i \<in> I. a i = b i}) [x] bs = [{i \<in> I. x i = y i}]\<close> and
+      \<open>{i \<in> I. x i = y i} \<in> F\<close> 
+      by simp+
+    then show ?case
+      by auto 
+  next
+    case (2 x xs)
+    then obtain y ys where
+      bs_is: \<open>bs = y # ys\<close> and
+      x_sym_y: \<open>(x, y) \<in> (\<sim>)\<close> and
+      \<open>list_all2 (in_rel (\<sim>)) xs ys\<close> and
+      \<open>length xs = length ys\<close>
+      by (smt (verit, best) in_rel_def list_all2_Cons1 list_all2_lengthD) 
+    then have \<open>\<Inter> (set (map2 (\<lambda> a b. {i \<in> I. a i = b i}) xs ys)) \<in> F\<close>
+      using "2.IH" "2.prems"(1)
+      by fastforce
+    moreover have \<open>{i \<in> I. x i = y i} \<in> F\<close>
+      using x_sym_y
+      by blast
+    ultimately have \<open>{i \<in> I. x i = y i} \<inter> \<Inter> (set (map2 (\<lambda> a b. {i \<in> I. a i = b i}) xs ys)) \<in> F\<close>
+      using filter.closed_int[OF F_filter]
+      by blast 
+    then show ?case
+      unfolding bs_is
+      by simp  
+  qed
+qed
+
+lemma inter_map2_to_set_compr:
+  assumes
+    \<open>as \<noteq> []\<close> and 
+    \<open>length as = length bs\<close> and
+    \<open>list_all2 (in_rel (\<sim>)) as bs\<close>
+  shows \<open>\<Inter> (set (map2 (\<lambda> a b. {i \<in> I. a i = b i}) as bs)) =
+    {i \<in> I. \<forall> (a, b) \<in> set (zip as bs). a i = b i}\<close>
+  using assms(2, 3)
+proof (induction arbitrary: bs rule: list_nonempty_induct[OF assms(1)])
+  case (1 x)
+  then obtain y where
+    bs_is: \<open>bs = [y]\<close> and
+    \<open>(x, y) \<in> (\<sim>)\<close>
+    by (metis (no_types, lifting) in_rel_def list_all2_Cons1 list_all2_Nil) 
+  then show ?case
+    unfolding bs_is
+    by simp 
+next
+  case (2 x xs)
+  then obtain y ys where
+    bs_is: \<open>bs = y # ys\<close> and
+    \<open>(x, y) \<in> (\<sim>)\<close> and
+    \<open>list_all2 (in_rel (\<sim>)) xs ys\<close> and
+    \<open>length xs = length ys\<close>
+    by (smt (verit, ccfv_SIG) in_rel_def list_all2_Cons1 list_all2_lengthD) 
+  then have \<open>\<Inter> (set (map2 (\<lambda> x y. {i \<in> I. x i = y i}) xs ys)) =
+    {i \<in> I. \<forall> (a, b) \<in> set (zip xs ys). a i = b i}\<close>
+    using "2.IH"
+    by presburger
+  then have \<open>{i \<in> I. x i = y i} \<inter> \<Inter> (set (map2 (\<lambda> x y. {i \<in> I. x i = y i}) xs ys)) =
+    {i \<in> I. x i = y i} \<inter> {i \<in> I. \<forall> (a, b) \<in> set (zip xs ys). a i = b i}\<close>
+    by blast 
+  moreover have \<open>{i \<in> I. x i = y i} \<inter> \<Inter> (set (map2 (\<lambda> x y. {i \<in> I. x i = y i}) xs ys)) =
+    \<Inter> (set (map2 (\<lambda> x y. {i \<in> I. x i = y i}) (x # xs) (y # ys)))\<close>
+    by simp 
+  moreover have \<open>{i \<in> I. x i = y i} \<inter> {i \<in> I. \<forall> (a, b) \<in> set (zip xs ys). a i = b i} =
+    {i \<in> I. \<forall> (a, b) \<in> set (zip (x # xs) (y # ys)). a i = b i}\<close>
+  proof -
+    have \<open>{i \<in> I. x i = y i} \<inter> {i \<in> I. \<forall> (a, b) \<in> set (zip xs ys). a i = b i} =
+      {i \<in> I. x i = y i \<and> (\<forall> (a, b) \<in> set (zip xs ys). a i = b i)}\<close>
+      by blast
+    also have \<open>... = {i \<in> I. \<forall> (a, b) \<in> set (zip (x # xs) (y # ys)). a i = b i}\<close>
+      by auto 
+    finally show ?thesis . 
+  qed
+  ultimately show ?case
+    unfolding bs_is
+    by simp 
+qed 
+
+lemma well_definedness_REL:
+  assumes
+    \<open>length as = length bs\<close> and
+    \<open>list_all2 (in_rel (\<sim>)) as bs\<close>
+  shows
+    \<open>{i \<in> I. [a i. a \<leftarrow> as] \<in> interp_rel (\<M> i) p} \<in> F \<longleftrightarrow>
+       {i \<in> I. [b i. b \<leftarrow> bs] \<in> interp_rel (\<M> i) p} \<in> F\<close>
+proof (cases \<open>as = []\<close>) 
+  case True
+  then have \<open>bs = []\<close>
+    using assms(1)
+    by simp 
+  then show ?thesis
+    using True
+    by auto
+next
+  case False
+  then have bs_not_empty: \<open>bs \<noteq> []\<close>
+    using assms(1)
+    by auto
+
+  have dummy_A_in_F: \<open>\<Inter> (set (map2 (\<lambda> a b. {i \<in> I. a i = b i}) as bs)) \<in> F\<close>
+    (is \<open>?A \<in> _\<close>)
+    by (rule lists_related_to_inter_in_filter[OF False assms(1, 2)]) 
+
+  have dummy_A_is: \<open>?A = {i \<in> I. \<forall> (a, b) \<in> set (zip as bs). a i = b i}\<close>
+    by (fact inter_map2_to_set_compr[OF False assms(1, 2)]) 
+
+  let ?Pa = \<open>{i \<in> I. [a i. a \<leftarrow> as] \<in> interp_rel (\<M> i) p}\<close>
+  let ?Pb = \<open>{i \<in> I. [b i. b \<leftarrow> bs] \<in> interp_rel (\<M> i) p}\<close>
+
+  have Pa_inter_A_eq_Pb_inter_A: \<open>?Pa \<inter> ?A = ?Pb \<inter> ?A\<close>
+    unfolding dummy_A_is
+  proof -
+    have \<open>?Pa \<inter> {i \<in> I. \<forall> (a, b) \<in> set (zip as bs). a i = b i} =
+      {i \<in> I. [a i. a \<leftarrow> as] \<in> interp_rel (\<M> i) p \<and> (\<forall> (a, b) \<in> set (zip as bs). a i = b i)}\<close>
+      (is \<open>?lhs = _\<close>)
+      by fastforce 
+    also have
+      \<open>... = {i \<in> I. [b i. b \<leftarrow> bs] \<in> interp_rel (\<M> i) p \<and> (\<forall> (a, b) \<in> set (zip as bs). a i = b i)}\<close>
+      using assms(1, 2)
+    proof (induction arbitrary: bs rule: list_nonempty_induct[OF False])
+      case (1 x)
+      then obtain y where
+        bs_is: \<open>bs = [y]\<close> and
+        \<open>(x, y) \<in> (\<sim>)\<close>
+        by (metis (no_types, lifting) in_rel_def list_all2_Cons1 list_all2_Nil) 
+      then show ?case
+        unfolding bs_is
+        by fastforce 
+    next
+      case (2 x xs)
+      then obtain y ys where
+        bs_is: \<open>bs = y # ys\<close> and
+        \<open>(x, y) \<in> (\<sim>)\<close> and
+        \<open>list_all2 (in_rel (\<sim>)) xs ys\<close> and
+        len_eq: \<open>length xs = length ys\<close>
+        by (smt (verit, best) in_rel_def list_all2_Cons1 list_all2_lengthD) 
+      then have
+        \<open>{i \<in> I. [a i. a \<leftarrow> xs] \<in> interp_rel (\<M> i) p \<and> (\<forall> (a, b) \<in> set (zip xs ys). a i = b i)} =
+        {i \<in> I. [b i. b \<leftarrow> ys] \<in> interp_rel (\<M> i) p \<and> (\<forall> (a, b) \<in> set (zip xs ys). a i = b i)}\<close>
+        using "2.IH"
+        by presburger
+
+      show ?case
+        unfolding bs_is
+      proof (intro subset_antisym subsetI; clarsimp)
+        fix i
+        assume
+          \<open>i \<in> I\<close> and
+          \<open>(y i # map (\<lambda> a. a i) xs) \<in> interp_rel (\<M> i) p\<close> and 
+          \<open>x i = y i\<close> and 
+          \<open>\<forall> (a, b) \<in> set (zip xs ys). a i = b i\<close>
+        then show \<open>(y i # map (\<lambda> b. b i) ys) \<in> interp_rel (\<M> i) p\<close>
+          using len_eq
+        proof (induction xs ys rule: list_induct2')
+          case (4 x' xs' y' ys')
+          then have \<open>list_all2 (\<lambda> a b. a i = b i) (x' # xs') (y' # ys')\<close>
+            by (meson list_all2I)
+          then have \<open>[b i. b \<leftarrow> y' # ys'] = [a i. a \<leftarrow> x' # xs']\<close>
+            unfolding list_all2_iff_eq_maps[OF "4.prems"(5)] 
+            by simp 
+          then show ?case
+            using "4.prems"(2)
+            by presburger
+        qed auto 
+      next
+        fix i
+        assume
+          \<open>i \<in> I\<close> and
+          \<open>(y i # map (\<lambda> a. a i) ys) \<in> interp_rel (\<M> i) p\<close> and 
+          \<open>x i = y i\<close> and 
+          \<open>\<forall> (a, b) \<in> set (zip xs ys). a i = b i\<close>
+        then show \<open>(y i # map (\<lambda> b. b i) xs) \<in> interp_rel (\<M> i) p\<close>
+          using len_eq 
+        proof (induction xs ys rule: list_induct2')
+          case (4 x' xs' y' ys')
+          then have \<open>list_all2 (\<lambda> a b. a i = b i) (x' # xs') (y' # ys')\<close>
+            by (meson list_all2I) 
+          then have \<open>[b i. b \<leftarrow> y' # ys'] = [a i. a \<leftarrow> x' # xs']\<close>
+            unfolding list_all2_iff_eq_maps[OF "4.prems"(5)]
+            by simp 
+          then show ?case
+            using "4.prems"(2)
+            by presburger
+        qed auto 
+      qed
+    qed
+    also have
+      \<open>... = ?Pb \<inter> {i \<in> I. \<forall> (a, b) \<in> set (zip as bs). a i = b i}\<close>
+      (is \<open>_ = ?rhs\<close>)
+      by fastforce 
+    finally show \<open>?lhs = ?rhs\<close> .
+  qed
+  then show \<open>?Pa \<in> F \<longleftrightarrow> ?Pb \<in> F\<close>
+    using filter.closed_int[OF F_filter] filter.upwards_closed[OF F_filter]
+    by (smt (verit, ccfv_threshold) CollectD dummy_A_in_F inf_le1 subset_eq) 
+  (* proof (intro iffI)
+   *   assume \<open>?Pa \<in> F\<close>
+   *   then have \<open>?Pa \<inter> ?A \<in> F\<close>
+   *     using filter.closed_int[OF F_filter _ dummy_A_in_F]
+   *     by blast 
+   *   moreover have \<open>?Pa \<inter> ?A \<subseteq> ?Pb\<close>
+   *     using Pa_inter_A_eq_Pb_inter_A
+   *     by blast  
+   *   ultimately show \<open>?Pb \<in> F\<close>
+   *     using filter.upwards_closed[OF F_filter]
+   *     by (metis (no_types, lifting) CollectD F_filter filter.in_F_subset_S subsetI) 
+   * next
+   *   assume \<open>?Pb \<in> F\<close>
+   *   then have \<open>?Pb \<inter> ?A \<in> F›
+   *     using filter.closed_int[OF F_filter _ dummy_A_in_F]
+   *     by blast
+   *   moreover have \<open>?Pb \<inter> ?A \<subseteq> ?Pa\<close>
+   *     using Pa_inter_A_eq_Pb_inter_A
+   *     by blast 
+   *   ultimately show \<open>?Pa \<in> F\<close>
+   *     using filter.upwards_closed[OF F_filter]
+   *     by (metis (no_types, lifting) CollectD F_filter filter.in_F_subset_S subsetI) 
+   * qed *)
+qed
+
+lemma well_definedness_FN:
+  assumes
+    \<open>length as = length bs\<close> and
+    \<open>list_all2 (in_rel (\<sim>)) as bs\<close>
+  shows
+    \<open>(\<sim>) `` {\<lambda> i \<in> I. interp_fn (\<M> i) f [a i. a \<leftarrow> as]} =
+       (\<sim>) `` {\<lambda> i \<in> I. interp_fn (\<M> i) f [b i. b \<leftarrow> bs]}\<close>
+proof (cases \<open>as = []\<close>) 
+  case True
+  then have \<open>bs = []\<close>
+    using assms(1)
+    by simp 
+  then show ?thesis
+    using True
+    by fastforce 
+next
+  case False
+
+  have
+    all_as_in_Pi: \<open>list_all (\<lambda> a. a \<in> (\<Pi> i \<in> I. dom (\<M> i))) as\<close> and
+    all_bs_in_Pi: \<open>list_all (\<lambda> b. b \<in> (\<Pi> i \<in> I. dom (\<M> i))) bs\<close>
+    using assms(1, 2)
+    by (induction as bs rule: list_induct2', auto) 
+
+  have \<open>{i \<in> I. interp_fn (\<M> i) f [a i. a \<leftarrow> as] = interp_fn (\<M> i) f [b i. b \<leftarrow> bs]} \<in> F\<close>
+  proof - 
+    have dummy_A_in_F: \<open>\<Inter> (set (map2 (\<lambda> a b. {i \<in> I. a i = b i}) as bs)) \<in> F\<close>
+      (is \<open>?A \<in> _\<close>)
+      by (fact lists_related_to_inter_in_filter[OF False assms(1, 2)]) 
+
+    have dummy_A_is: \<open>?A = {i \<in> I. \<forall> (a, b) \<in> set (zip as bs). a i = b i}\<close>
+      (is \<open>_ = ?B\<close>)
+      by (fact inter_map2_to_set_compr[OF False assms(1, 2)]) 
+    then have \<open>?B \<in> F\<close>
+      using dummy_A_in_F
+      by fastforce
+    moreover have \<open>?B \<subseteq> {i \<in> I. [a i. a \<leftarrow> as] = [b i. b \<leftarrow> bs]}\<close>
+      using assms(1) 
+      by (induct as bs rule: list_induct2', auto)
+    ultimately have \<open>{i \<in> I. [a i. a \<leftarrow> as] = [b i. b \<leftarrow> bs]} \<in> F\<close>
+      using filter.upwards_closed[OF F_filter]
+      by (metis (mono_tags, lifting) CollectD subsetI) 
+    moreover have
+      \<open>{i \<in> I. [a i. a \<leftarrow> as] = [b i. b \<leftarrow> bs]} \<subseteq>
+       {i \<in> I. interp_fn (\<M> i) f [a i. a \<leftarrow> as] = interp_fn (\<M> i) f [b i. b \<leftarrow> bs]}\<close>
+      by auto 
+    ultimately show ?thesis
+      using filter.upwards_closed[OF F_filter] 
+      by (metis (no_types, lifting) CollectD subsetI) 
+  qed
+  moreover have \<open>(\<lambda> i \<in> I. interp_fn (\<M> i) f [a i. a \<leftarrow> as]) \<in> (\<Pi> i \<in> I. dom (\<M> i))\<close>
+  proof -
+    have \<open>list_all (\<lambda> a. a \<in> (\<Pi> i \<in> I. dom (\<M> i))) as\<close>
+      by (fact all_as_in_Pi)
+    then have \<open>list_all (\<lambda> a. a i \<in> dom (\<M> i)) as\<close>
+      if \<open>i \<in> I\<close>
+      for i
+      by (metis (no_types, lifting) PiE list.pred_mono_strong that) 
+    then have \<open>interp_fn (\<M> i) f [a i. a \<leftarrow> as] \<in> dom (\<M> i)\<close>
+      if \<open>i \<in> I\<close>
+      for i
+      using
+        struct.FN_dom_to_dom[OF struct_Mi[rule_format, OF that], rule_format, of \<open>[a i. a \<leftarrow> as]\<close> f]
+      by (smt (verit, del_insts) imageE list.pred_set list.set_map that) 
+    then show ?thesis
+      by blast 
+  qed
+  moreover have \<open>(\<lambda> i \<in> I. interp_fn (\<M> i) f [b i. b \<leftarrow> bs]) \<in> (\<Pi> i \<in> I. dom (\<M> i))\<close>
+  proof -
+    have \<open>list_all (\<lambda> b. b \<in> (\<Pi> i \<in> I. dom (\<M> i))) bs\<close>
+      by (fact all_bs_in_Pi)
+    then have \<open>list_all (\<lambda> b. b i \<in> dom (\<M> i)) bs\<close>
+      if \<open>i \<in> I\<close>
+      for i
+      by (metis (no_types, lifting) PiE list.pred_mono_strong that) 
+    then have \<open>interp_fn (\<M> i) f [b i. b \<leftarrow> bs] \<in> dom (\<M> i)\<close>
+      if \<open>i \<in> I\<close>
+      for i
+      using
+        struct.FN_dom_to_dom[OF struct_Mi[rule_format, OF that], rule_format, of \<open>[b i. b \<leftarrow> bs]\<close> f]
+      by (smt (verit, del_insts) imageE list.pred_set list.set_map that) 
+    then show ?thesis
+      by blast 
+  qed
+  ultimately have
+    \<open>(\<lambda> i \<in> I. interp_fn (\<M> i) f [a i. a \<leftarrow> as], \<lambda> i \<in> I. interp_fn (\<M> i) f [b i. b \<leftarrow> bs]) \<in> (\<sim>)\<close>
+    by (smt (verit, best) Collect_cong case_prodI mem_Collect_eq restrict_apply') 
+
+  then show ?thesis
+    unfolding equiv_class_eq_iff[OF equiv_prod_eq]
+    by fastforce 
+qed
+
+lemma fun_upd_rep_is_rep_fun_upd: \<open>(\<lambda> v. rep (\<beta> v) i)(x := rep a i) = (\<lambda> v. rep ((\<beta>(x := a)) v) i)\<close>
+proof -
+  have \<open>(\<lambda> v. rep (\<beta> v) i)(x := rep a i) = (\<lambda> v. if v = x then rep a i else rep (\<beta> v) i)\<close>
+    by fastforce 
+  also have \<open>... = (\<lambda> v. (if v = x then rep a else rep (\<beta> v)) i)\<close>
+    by fastforce  
+  also have \<open>... = (\<lambda> v. rep (if x = v then a else \<beta> v) i)\<close>
+    by fastforce 
+  also have \<open>... = (\<lambda> v. rep ((\<beta>(x := a)) v) i)\<close>
+    by fastforce 
+  finally show ?thesis . 
+qed
+
+lemma lam_i_eval_in_Pi:
+  assumes \<open>is_vars (dom \<A>) \<beta>\<close> 
+  shows \<open>(\<lambda> i \<in> I. \<lbrakk>t\<rbrakk>\<^bsup>\<M> i,\<lambda> v. rep (\<beta> v) i\<^esup>) \<in> (\<Pi> i \<in> I. dom (\<M> i))\<close>
+proof (induction t) 
+  case (Var v)
+  then show ?case
+    using assms
+    unfolding is_vars_def
+    using equiv_Eps_preserves[OF equiv_prod_eq] rep_def rep_of_elem_ultraproduct_in_pi
+    by fastforce
+next
+  case (Fun f ts)
+
+  have \<open>\<lbrakk>Fun f ts\<rbrakk>\<^bsup>\<M> i,\<lambda>v. rep (\<beta> v) i\<^esup> = interp_fn (\<M> i) f [\<lbrakk>t\<rbrakk>\<^bsup>\<M> i,\<lambda> v. rep (\<beta> v) i\<^esup>. t \<leftarrow> ts]\<close>
+    if \<open>i \<in> I\<close>
+    for i
+    by simp 
+  moreover have \<open>\<lbrakk>t\<rbrakk>\<^bsup>\<M> i,\<lambda> v. rep (\<beta> v) i\<^esup> \<in> dom (\<M> i)\<close>
+    if
+      \<open>i \<in> I\<close> and
+      \<open>t \<in> set ts\<close>
+    for i t
+    using Fun[OF that(2)]
+    by (meson PiE restrict_Pi_cancel that(1)) 
+  then have \<open>\<forall> t \<in> set ts. \<lbrakk>t\<rbrakk>\<^bsup>\<M> i,\<lambda> v. rep (\<beta> v) i\<^esup> \<in> dom (\<M> i)\<close>
+    if \<open>i \<in> I\<close>
+    for i
+    using that
+    by blast
+  then have \<open>interp_fn (\<M> i) f [\<lbrakk>t\<rbrakk>\<^bsup>\<M> i,\<lambda> v. rep (\<beta> v) i\<^esup>. t \<leftarrow> ts] \<in> dom (\<M> i)\<close>
+    if \<open>i \<in> I\<close>
+    for i
+    using struct.FN_dom_to_dom[OF struct_Mi[rule_format, OF that]] that 
+    by simp 
+  ultimately show ?case
+    by force
+qed
+
+lemma eval_\<UU>_is_eq_class:
+  assumes \<open>is_vars (dom \<A>) \<beta>\<close> 
+  shows \<open>\<lbrakk>t\<rbrakk>\<^bsup>\<A>,\<beta>\<^esup> = (\<sim>) `` {\<lambda> i \<in> I. \<lbrakk>t\<rbrakk>\<^bsup>\<M> i,\<lambda> v. rep (\<beta> v) i\<^esup>}\<close>
+proof (induction t) 
+  case (Var v)
+
+  have \<open>\<lbrakk>Var v\<rbrakk>\<^bsup>\<A>,\<beta>\<^esup> = \<beta> v\<close>
+    by simp 
+  moreover
+  {
+    have \<open>(\<lambda> i \<in> I. \<lbrakk>Var v\<rbrakk>\<^bsup>\<M> i,\<lambda> v. rep (\<beta> v) i\<^esup>) = (\<lambda> i \<in> I. rep (\<beta> v) i)\<close>
+      by auto 
+    then have
+      \<open>(\<sim>) `` {\<lambda> i \<in> I. \<lbrakk>Var v\<rbrakk>\<^bsup>\<M> i,\<lambda> v. rep (\<beta> v) i\<^esup>} = (\<sim>) `` {\<lambda> i \<in> I. rep (\<beta> v) i}\<close>
+      by argo
+    also have \<open>... = \<beta> v\<close>
+    proof -
+      have \<open>(\<lambda> i \<in> I. rep (\<beta> v) i, rep (\<beta> v)) \<in> (\<sim>)\<close>
+        by (smt (verit, ccfv_SIG) Collect_cong assms case_prodD case_prodI dom_\<A> is_vars_def
+            mem_Collect_eq refl_onD refl_prod_eq rep_of_elem_ultraproduct_in_pi restrict_Pi_cancel
+            restrict_apply') 
+      then have \<open>(\<sim>) `` {\<lambda> i \<in> I. rep (\<beta> v) i} = (\<sim>) `` {rep (\<beta> v)}\<close>
+        by (metis (no_types, lifting) equiv_class_eq_iff equiv_prod_eq) 
+      also have \<open>... = \<beta> v\<close>
+        by (smt (verit, best) assms dom_\<A> elem_eq_class_in_pi equiv_class_eq_iff equiv_prod_eq
+            is_vars_def quotientE rep_relates_to_elem_of_equiv_class) 
+      finally show ?thesis .
+    qed
+    finally have \<open>(\<sim>) `` {\<lambda> i \<in> I. \<lbrakk>Var v\<rbrakk>\<^bsup>\<M> i,\<lambda> v. rep (\<beta> v) i\<^esup>} = \<beta> v\<close> . 
+  }
+  ultimately show ?case .. 
+next
+  case (Fun f ts)
+ 
+  have \<open>\<lbrakk>Fun f ts\<rbrakk>\<^bsup>\<A>,\<beta>\<^esup> = FN f [\<lbrakk>t\<rbrakk>\<^bsup>\<A>,\<beta>\<^esup>. t \<leftarrow> ts]\<close>
+    using interp_fn_\<A> 
+    by simp
+  also have \<open>... = (\<sim>) `` {\<lambda> i \<in> I. interp_fn (\<M> i) f [rep e i. e \<leftarrow> [\<lbrakk>t\<rbrakk>\<^bsup>\<A>,\<beta>\<^esup>. t \<leftarrow> ts]]}\<close>
+    unfolding FN_def
+    by blast 
+  also have \<open>... = (\<sim>) `` {\<lambda> i \<in> I. interp_fn (\<M> i) f [rep (\<lbrakk>t\<rbrakk>\<^bsup>\<A>,\<beta>\<^esup>) i. t \<leftarrow> ts]}\<close>
+    unfolding map_map_is_map ..
+  also have \<open>... = (\<sim>) `` {\<lambda> i \<in> I. interp_fn (\<M> i) f
+    [rep ((\<sim>) `` {\<lambda> i \<in> I. \<lbrakk>t\<rbrakk>\<^bsup>\<M> i,\<lambda> v. rep (\<beta> v) i\<^esup>}) i. t \<leftarrow> ts]}\<close>
+    using Fun.IH
+    by (smt (verit, ccfv_SIG) map_eq_conv restrict_ext) 
+  also have
+    \<open>... = (\<sim>) `` {\<lambda> i \<in> I. interp_fn (\<M> i) f [(\<lambda> i \<in> I. ⟦t\<rbrakk>\<^bsup>\<M> i,\<lambda> v. rep (\<beta> v) i\<^esup>) i. t \<leftarrow> ts]}\<close>
+  proof -
+    let ?as = \<open>[rep ((\<sim>) `` {\<lambda> i \<in> I. \<lbrakk>t\<rbrakk>\<^bsup>\<M> i,\<lambda> v. rep (\<beta> v) i\<^esup>}). t \<leftarrow> ts]\<close>
+    let ?bs = \<open>[(\<lambda> i \<in> I. \<lbrakk>t\<rbrakk>\<^bsup>\<M> i,\<lambda> v. rep (\<beta> v) i\<^esup>). t \<leftarrow> ts]\<close>
+
+    have len_eq: \<open>length ?as = length ?bs\<close>
+      by auto 
+    then have \<open>list_all2 (in_rel (\<sim>)) ?as ?bs\<close>
+    proof (induction ts) 
+      case (Cons t ts)
+
+      have \<open>(rep ((\<sim>) `` {\<lambda> i \<in> I. \<lbrakk>t\<rbrakk>\<^bsup>\<M> i,\<lambda> v. rep (\<beta> v) i\<^esup>}),
+        (\<lambda> i \<in> I. \<lbrakk>t\<rbrakk>\<^bsup>\<M> i,\<lambda> v. rep (\<beta> v) i\<^esup>)) \<in> (\<sim>)\<close>
+        using lam_i_eval_in_Pi[OF assms, of t] rep_relates_to_elem_of_equiv_class
+        by presburger 
+      moreover have \<open>list_all2 (in_rel (\<sim>))
+        [rep ((\<sim>) `` {\<lambda> i \<in> I. \<lbrakk>t\<rbrakk>\<^bsup>\<M> i,\<lambda> v. rep (\<beta> v) i\<^esup>}). t \<leftarrow> ts]
+        [(\<lambda> i \<in> I. \<lbrakk>t\<rbrakk>\<^bsup>\<M> i,\<lambda> v. rep (\<beta> v) i\<^esup>). t \<leftarrow> ts]\<close>
+        using Cons
+        by fastforce 
+      ultimately show ?case
+        by (smt (z3) in_rel_def list.simps(9) list_all2_Cons1 restrict_ext) 
+    qed auto 
+    then have
+      \<open>(\<sim>) `` {\<lambda> i \<in> I. interp_fn (\<M> i) f [e\<^sub>i i. e\<^sub>i \<leftarrow> ?as]} =
+        (\<sim>) `` {\<lambda> i \<in> I. interp_fn (\<M> i) f [e\<^sub>i i. e\<^sub>i \<leftarrow> ?bs]}\<close>
+      using well_definedness_FN[OF len_eq]
+      by meson 
+    then show ?thesis
+      unfolding map_map_is_map2 .
+  qed
+  also have \<open>... = (\<sim>) `` {\<lambda> i \<in> I. interp_fn (\<M> i) f [\<lbrakk>t\<rbrakk>\<^bsup>\<M> i,\<lambda> v. rep (\<beta> v) i\<^esup>. t \<leftarrow> ts]}\<close>
+    by force 
+  also have \<open>... = (\<sim>) `` {\<lambda> i \<in> I. \<lbrakk>Fun f ts\<rbrakk>\<^bsup>\<M> i,\<lambda> v. rep (\<beta> v) i\<^esup>}\<close>
+    by auto 
+  finally show ?case . 
+qed
+
+lemma some_i_in_Mi: 
+  assumes
+    \<open>a \<in> A\<close> and
+    \<open>i \<in> I\<close>
+  shows \<open>(\<some> y. y \<in> a) i \<in> dom (\<M> i)\<close>
+  using assms(1) assms(2) equiv_Eps_preserves equiv_prod_eq
+  by fastforce
+
+lemma in_filter_ex_if_ex_in_filter:
+  shows 
+    \<open>(\<exists> a \<in> dom \<A>. {i \<in> I. \<M> i,(\<lambda> v. rep (\<beta> v) i)(x := rep a i) \<Turnstile> \<phi>} \<in> F) \<Longrightarrow>
+      {i \<in> I. \<exists> a \<in> dom (\<M> i). \<M> i,(\<lambda> v. rep (\<beta> v) i)(x := a) \<Turnstile> \<phi>} \<in> F\<close>
+    (is \<open>?lhs \<Longrightarrow> ?rhs\<close>)
+proof -
+  assume ?lhs
+  then obtain a where
+    a_in_A: \<open>a \<in> dom \<A>\<close> and
+    \<open>{i \<in> I. \<M> i,(\<lambda> v. rep (\<beta> v) i)(x := rep a i) \<Turnstile> \<phi>} \<in> F\<close>
+    by blast
+  then have \<open>{i \<in> I. \<M> i,(\<lambda> v. rep (\<beta> v) i)(x := (\<some> y. y \<in> a) i) \<Turnstile> \<phi>} \<in> F\<close>
+    unfolding rep_def
+    by blast
+  moreover have \<open>\<M> i,(\<lambda> v. rep (\<beta> v) i)(x := (\<some> y. y \<in> a) i) \<Turnstile> \<phi>\<close> 
+    if
+      \<open>\<M> i,(\<lambda> v. rep (\<beta> v) i)(x := rep a i) \<Turnstile> \<phi>\<close> and
+      \<open>i \<in> I\<close>
+    for i
+    using rep_def that(1)
+    by force
+  then have \<open>{i \<in> I. \<M> i,(\<lambda> v. rep (\<beta> v) i)(x := rep a i) \<Turnstile> \<phi>} \<subseteq>
+    {i \<in> I. \<M> i,(\<lambda> v. rep (\<beta> v) i)(x := (\<some> y. y \<in> a) i) \<Turnstile> \<phi>}\<close>
+    using Collect_mono_iff
+    by blast 
+  moreover have \<open>a \<in> A\<close>
+    using a_in_A
+    by (subst (asm) dom_\<A>) 
+  ultimately show ?rhs
+    using filter.upwards_closed[OF F_filter, of \<open>{i \<in> I. \<M> i,(\<lambda>v. rep (\<beta> v) i)
+      (x := (SOME y. y \<in> a) i) \<Turnstile> \<phi>}\<close>]
+    by (smt (verit, best) Eps_cong Pi_iff mem_Collect_eq rep_def rep_of_elem_ultraproduct_in_pi
+        subsetI) 
+qed 
+
+lemma inline_restrict_in_set_compr:
+  \<open>{i \<in> I. P [(\<lambda> i \<in> I. f g i) i. g \<leftarrow> L]} = {i \<in> I. P [f g i. g \<leftarrow> L]}\<close>
+  by force 
+
+abbreviation (input) I_fm :: \<open>('f, 'p, 'v) fm \<Rightarrow> ('v \<Rightarrow> ('i \<Rightarrow> 'm) set) \<Rightarrow> 'i set\<close> (\<open>I\<^bsub>_\<^esub>\<^bsup>_\<^esup>\<close>) where
+  \<open>I\<^bsub>\<chi>\<^esub>\<^bsup>\<beta>\<^esup> \<equiv> {i \<in> I. \<M> i,(\<lambda> v. rep (\<beta> v) i) \<Turnstile> \<chi>}\<close>
+
+(* Theorem 3.1 *)
+theorem los:
+  assumes \<open>is_vars (dom \<A>) \<beta>\<close>
+    \<comment>\<open>This assumption is crucial because we don't want to consider cases where \<open>\<beta>\<close> maps variables
+      to equivalence classes on a relation other than @{const prod_eq}.
+      Ideally, this would have been a restriction on the type of \<open>\<beta>\<close> but this doesn't seem to be
+      possible in Isabelle.\<close>
+  shows \<open>\<A>,\<beta> \<Turnstile> \<phi> \<longleftrightarrow> I\<^bsub>\<phi>\<^esub>\<^bsup>\<beta>\<^esup> \<in> F\<close>
+  using assms
+proof (induction \<phi> arbitrary: \<beta>) 
+  case (Rel p e)
+
+  have \<open>\<A>,\<beta> \<Turnstile> Rel p e \<longleftrightarrow> [\<lbrakk>t\<rbrakk>\<^bsup>\<A>,\<beta>\<^esup>. t \<leftarrow> e] \<in> REL p\<close> (is \<open>_ \<longleftrightarrow> ?e \<in> _\<close>)
+    using interp_rel_\<A>
+    by auto 
+  also have
+    \<open>... \<longleftrightarrow> (\<forall> x \<in> set ?e. x \<in> A) \<and> {i \<in> I. [rep e\<^sub>i i. e\<^sub>i \<leftarrow> ?e] \<in> interp_rel (\<M> i) p} \<in> F\<close>
+    unfolding REL_def
+    by blast 
+  also have
+    \<open>... \<longleftrightarrow> (\<forall> x \<in> set ?e. x \<in> A) \<and> {i \<in> I. [rep (\<lbrakk>t\<rbrakk>\<^bsup>\<A>,\<beta>\<^esup>) i. t \<leftarrow> e] \<in> interp_rel (\<M> i) p} \<in> F\<close>
+    unfolding map_map_is_map
+    by blast
+  also have \<open>... \<longleftrightarrow> (\<forall> x \<in> set ?e. x \<in> A) \<and> {i \<in> I. 
+    [rep ((\<sim>) `` {\<lambda> i \<in> I. \<lbrakk>t\<rbrakk>\<^bsup>\<M> i,\<lambda> v. rep (\<beta> v) i\<^esup>}) i. t \<leftarrow> e] \<in> interp_rel (\<M> i) p} \<in> F\<close>
+    using eval_\<UU>_is_eq_class[OF Rel.prems(1)]
+    by simp 
+  also have \<open>... \<longleftrightarrow> (\<forall> x \<in> set ?e. x \<in> A) \<and>
+    {i \<in> I. [\<lbrakk>t\<rbrakk>\<^bsup>\<M> i,\<lambda> v. rep (\<beta> v) i\<^esup>. t \<leftarrow> e] \<in> interp_rel (\<M> i) p} \<in> F\<close>
+  proof -
+    let ?as = \<open>[rep ((\<sim>) `` {\<lambda> i \<in> I. \<lbrakk>t\<rbrakk>\<^bsup>\<M> i,\<lambda> v. rep (\<beta> v) i\<^esup>}). t \<leftarrow> e]\<close> 
+    let ?bs = \<open>[(\<lambda> i \<in> I. \<lbrakk>t\<rbrakk>\<^bsup>\<M> i,\<lambda> v. rep (\<beta> v) i\<^esup>). t \<leftarrow> e]\<close>
+
+    have len_eq: \<open>length ?as = length ?bs\<close>
+      by simp 
+    then have \<open>list_all2 (in_rel (\<sim>)) ?as ?bs\<close>
+    proof (induction e)
+      case (Cons e es)
+
+      have \<open>(rep ((\<sim>) `` {\<lambda> i \<in> I. \<lbrakk>e\<rbrakk>\<^bsup>\<M> i,\<lambda> v. rep (\<beta> v) i\<^esup>}),
+        \<lambda> i \<in> I. \<lbrakk>e\<rbrakk>\<^bsup>\<M> i,\<lambda> v. rep (\<beta> v) i\<^esup>) \<in> (\<sim>)\<close>
+        using lam_i_eval_in_Pi[OF Rel.prems(1), of e] rep_relates_to_elem_of_equiv_class
+        by presburger 
+      moreover have \<open>list_all2 (in_rel (\<sim>))
+        [rep ((\<sim>) `` {\<lambda> i \<in> I. \<lbrakk>t\<rbrakk>\<^bsup>\<M> i,\<lambda> v. rep (\<beta> v) i\<^esup>}). t \<leftarrow> es]
+        [(\<lambda> i \<in> I. \<lbrakk>t\<rbrakk>\<^bsup>\<M> i,\<lambda> v. rep (\<beta> v) i\<^esup>). t \<leftarrow> es]\<close>
+        using Cons
+        by fastforce 
+      ultimately show ?case
+        by (smt (verit, ccfv_SIG) in_rel_def list.simps(9) list_all2_Cons1 restrict_ext) 
+    qed auto 
+    then have
+      \<open>{i \<in> I. [e\<^sub>i i. e\<^sub>i \<leftarrow> ?as] \<in> interp_rel (\<M> i) p} \<in> F \<longleftrightarrow>
+       {i \<in> I. [e\<^sub>i i. e\<^sub>i \<leftarrow> ?bs] \<in> interp_rel (\<M> i) p} \<in> F\<close>
+      using well_definedness_REL[OF len_eq]
+      by blast 
+    then show ?thesis
+      unfolding map_map_is_map2
+      by (intro iffI conjI; blast?)
+         (smt (verit, ccfv_threshold) Collect_cong map_eq_conv restrict_apply)+
+  qed
+  also have \<open>... \<longleftrightarrow> I\<^bsub>Rel p e\<^esub>\<^bsup>\<beta>\<^esup> \<in> F\<close>
+  proof -
+    have \<open>\<lbrakk>t\<rbrakk>\<^bsup>\<A>,\<beta>\<^esup> \<in> dom \<A>\<close>
+      if \<open>t \<in> set e\<close> 
+      for t 
+      using lam_i_eval_in_Pi[OF Rel.prems] eval_\<UU>_is_eq_class[OF Rel.prems] dom_\<A> that
+      by (smt (verit, ccfv_threshold) Pi_iff comp_apply quotientI) 
+    then show ?thesis
+      using quotientI dom_\<A> interp_rel_\<A>
+      by auto
+  qed
+  finally show ?case .
+next
+  case (Negation \<phi>)
+
+  have \<open>\<A>,\<beta> \<Turnstile> \<^bold>\<not> \<phi> \<longleftrightarrow> \<not> \<A>,\<beta> \<Turnstile> \<phi>\<close>
+    by auto 
+  also have \<open>... \<longleftrightarrow> I\<^bsub>\<phi>\<^esub>\<^bsup>\<beta>\<^esup> \<notin> F\<close>
+    using Negation.IH[OF Negation.prems(1)]
+    by blast
+  also have \<open>... \<longleftrightarrow> I - I\<^bsub>\<phi>\<^esub>\<^bsup>\<beta>\<^esup> \<in> F\<close>
+    using ultrafilter.maximality[OF F_ultrafilter, of \<open>I\<^bsub>\<phi>\<^esub>\<^bsup>\<beta>\<^esup>\<close>]
+    by (metis (mono_tags, lifting) CollectD Diff_disjoint F_filter filter.closed_int
+        filter.empty_not_in_F subsetI) 
+  also have \<open>... \<longleftrightarrow> {i \<in> I. \<not> \<M> i,(\<lambda> v. rep (\<beta> v) i) \<Turnstile> \<phi>} \<in> F\<close>
+    by (smt (verit) Collect_cong Diff_iff mem_Collect_eq minus_set_def) 
+  also have \<open>... \<longleftrightarrow> I\<^bsub>\<^bold>\<not> \<phi>\<^esub>\<^bsup>\<beta>\<^esup> \<in> F\<close>
+    by auto 
+  finally show ?case . 
+next
+  case (Conjunction \<phi> \<psi>)
+
+  have \<open>\<A>,\<beta> \<Turnstile> \<phi> \<^bold>\<and> \<psi> \<longleftrightarrow> \<A>,\<beta> \<Turnstile> \<phi> \<and> \<A>,\<beta> \<Turnstile> \<psi>\<close>
+    by auto 
+  also have \<open>... \<longleftrightarrow> I\<^bsub>\<phi>\<^esub>\<^bsup>\<beta>\<^esup> \<in> F \<and> I\<^bsub>\<psi>\<^esub>\<^bsup>\<beta>\<^esup> \<in> F\<close>
+    using Conjunction.IH[OF Conjunction.prems(1)]
+    by blast 
+  also have \<open>... \<longleftrightarrow> I\<^bsub>\<phi>\<^esub>\<^bsup>\<beta>\<^esup> \<inter> I\<^bsub>\<psi>\<^esub>\<^bsup>\<beta>\<^esup> \<in> F\<close>
+    using filter.closed_int[OF F_filter, of \<open>I\<^bsub>\<phi>\<^esub>\<^bsup>\<beta>\<^esup>\<close> \<open>I\<^bsub>\<psi>\<^esub>\<^bsup>\<beta>\<^esup>\<close>]
+          filter.closed_int'[OF F_filter, of \<open>I\<^bsub>\<phi>\<^esub>\<^bsup>\<beta>\<^esup>\<close> \<open>I\<^bsub>\<psi>\<^esub>\<^bsup>\<beta>\<^esup>\<close>] 
+    by blast 
+  also have \<open>... \<longleftrightarrow> I\<^bsub>\<phi> \<^bold>\<and> \<psi>\<^esub>\<^bsup>\<beta>\<^esup> \<in> F\<close>
+    (* /!\ Very slow /!\ *)
+    by auto (smt (verit, del_insts) Collect_cong Collect_conj_eq)+
+  finally show ?case . 
+next
+  \<comment>\<open>See \<^url>\<open>http://www.maths.gla.ac.uk/~gbellamy/LMS/PrestNotes.pdf\<close> (p10) for the proof of this case.
+    It is not exactly the same underneath, but close enough.\<close>
+
+  case (Existential x \<phi>)
+
+  show ?case
+  proof (intro iffI)
+    assume \<open>\<A>,\<beta> \<Turnstile> (\<^bold>\<exists> x\<^bold>. \<phi>)\<close>
+    then have *: \<open>\<exists> a \<in> dom \<A>. \<A>,\<beta>(x := a) \<Turnstile> \<phi>\<close>
+      by auto 
+    then have \<open>\<exists> a \<in> dom \<A>. {i \<in> I. \<M> i,(\<lambda> v. rep ((\<beta>(x := a)) v) i) \<Turnstile> \<phi>} \<in> F\<close> 
+    proof -
+      obtain a where
+        a_in_A: \<open>a \<in> dom \<A>\<close> and
+        \<phi>_entailed: \<open>\<A>,\<beta>(x := a) \<Turnstile> \<phi>\<close>
+        using "*"
+        by blast
+      then have \<open>is_vars (dom \<A>) (\<beta>(x := a))\<close> 
+        using Existential.prems
+        by auto
+      then show ?thesis
+        using Existential.IH[of \<open>\<beta>(x := a)\<close>] \<phi>_entailed a_in_A 
+        by blast 
+    qed 
+    then have \<open>\<exists> a \<in> dom \<A>. {i \<in> I. \<M> i,(\<lambda> v. rep (\<beta> v) i)(x := rep a i) \<Turnstile> \<phi>} \<in> F\<close>
+      by (simp add: fun_upd_rep_is_rep_fun_upd)
+    then have \<open>{i \<in> I. \<exists> a \<in> dom (\<M> i). \<M> i,(\<lambda> v. rep (\<beta> v) i)(x := a) \<Turnstile> \<phi>} \<in> F\<close> 
+      using in_filter_ex_if_ex_in_filter
+      by fastforce 
+    then show \<open>I\<^bsub>\<^bold>\<exists> x\<^bold>. \<phi>\<^esub>\<^bsup>\<beta>\<^esup> \<in> F\<close>
+      by auto 
+  next
+    assume \<open>I\<^bsub>\<^bold>\<exists> x\<^bold>. \<phi>\<^esub>\<^bsup>\<beta>\<^esup> \<in> F\<close>
+    then have ex_unfolded:
+      \<open>{i \<in> I. \<exists> a \<in> dom (\<M> i). \<M> i,(\<lambda> v. rep (\<beta> v) i)(x := a) \<Turnstile> \<phi>} \<in> F\<close>
+      (is \<open>?K \<in> F\<close>) 
+      by auto
+    then have \<open>\<forall> i \<in> ?K. \<exists> a \<in> dom (\<M> i). \<M> i,(\<lambda> v. rep (\<beta> v) i)(x := a) \<Turnstile> \<phi>\<close>
+      by force
+    then have
+      \<open>\<exists> u. \<forall> i \<in> ?K. u i \<in> dom (\<M> i) \<and> (\<M> i,(\<lambda> v. rep (\<beta> v) i)(x := u i) \<Turnstile> \<phi>)\<close>
+      by meson
+    then obtain u_tmp where
+      u_tmp_in_dom: \<open>u_tmp \<in> (\<Pi> i \<in> ?K. dom (\<M> i))\<close> and
+      u_tmp_def: \<open>\<forall> i \<in> ?K. \<M> i,(\<lambda> v. rep (\<beta> v) i)(x := u_tmp i) \<Turnstile> \<phi>\<close>
+      by fastforce 
+    then have
+      \<open>\<exists> u. (\<forall> i \<in> I. u i \<in> dom (\<M> i)) \<and> (\<forall> i \<in> ?K. \<M> i,(\<lambda> v. rep (\<beta> v) i)(x := u i) \<Turnstile> \<phi>)\<close>
+    proof -
+      have \<open>\<forall> i \<in> ?K. u_tmp i \<in> dom (\<M> i)\<close>
+        using u_tmp_in_dom
+        by auto
+      moreover have \<open>\<forall> i \<in> I. dom (\<M> i) \<noteq> {}\<close>
+        using struct.M_nonempty struct_Mi
+        by blast
+      ultimately have \<open>\<exists> u. (\<forall> i \<in> ?K. u i = u_tmp i) \<and> (\<forall> i \<in> I - ?K. u i = (\<some> x. x \<in> dom (\<M> i)))\<close>
+      proof -
+        let ?u = \<open>\<lambda> i \<in> I. if i \<in> ?K then u_tmp i else (\<some> x. x \<in> dom (\<M> i))\<close>
+        have \<open>\<forall> i \<in> ?K. ?u i = u_tmp i\<close>
+          by auto 
+        moreover have \<open>\<forall> i \<in> I - ?K. ?u i = (\<some> x. x \<in> dom (\<M> i))\<close>
+          by auto 
+        ultimately show ?thesis
+          by blast 
+      qed
+      then obtain u where
+        u_eq_u_tmp: \<open>\<forall> i \<in> ?K. u i = u_tmp i\<close> and
+        u_arbitrary: \<open>\<forall> i \<in> I - ?K. u i = (\<some> x. x \<in> dom (\<M> i))\<close>
+        by blast
+          
+      have \<open>\<forall> i \<in> ?K. \<M> i,(\<lambda> v. rep (\<beta> v) i)(x := u i) \<Turnstile> \<phi>\<close>
+        using u_tmp_def u_eq_u_tmp 
+        by auto
+      moreover have \<open>I - ?K \<union> ?K = I\<close>
+        by blast
+      then have \<open>\<forall> i \<in> I. (i \<in> ?K \<longrightarrow> u i = u_tmp i) \<and> (i \<in> I - ?K \<longrightarrow> u i = (\<some> x. x \<in> dom (\<M> i)))\<close>
+        using u_arbitrary u_eq_u_tmp 
+        by blast
+      then have \<open>\<forall> i \<in> I. (i \<in> ?K \<longrightarrow> u i = u_tmp i) \<and> (i \<in> I - ?K \<longrightarrow> u i \<in> dom (\<M> i))\<close>
+        using some_i_in_Mi struct_Mi[rule_format, THEN struct.M_nonempty]
+        by (simp add: some_in_eq) 
+      then have \<open>\<forall> i \<in> I. u i \<in> dom (\<M> i)\<close>
+        using u_tmp_in_dom[unfolded Pi_iff]
+        by fastforce
+      ultimately show ?thesis
+        by blast
+    qed
+    then have
+      \<open>\<exists> u \<in> (\<Pi> i \<in> I. dom (\<M> i)). (\<forall> i \<in> ?K. \<M> i,(\<lambda> v. rep (\<beta> v) i)(x := u i) \<Turnstile> \<phi>)\<close>
+      by (auto intro: Pi_iff) 
+    then obtain u where
+      u_in_dom: \<open>u \<in> (\<Pi> i \<in> I. dom (\<M> i))\<close> and
+      u_def: \<open>\<forall> i \<in> ?K. \<M> i,(\<lambda> v. rep (\<beta> v) i)(x := u i) \<Turnstile> \<phi>\<close>
+      by blast 
+
+    define c where
+      \<open>c \<equiv> (\<sim>) `` {u}\<close>
+
+    have \<open>{i \<in> I. rep c i = u i} \<in> F\<close>
+      using rep_relates_to_elem_of_equiv_class[OF u_in_dom] c_def
+      by fastforce
+    then have
+      \<open>\<exists> I' \<subseteq> I. I' \<in> F \<and> (\<forall> i \<in> I'. \<M> i,(\<lambda> v. rep (\<beta> v) i)(x := rep c i) \<Turnstile> \<phi> \<longleftrightarrow>
+        \<M> i,(\<lambda> v. rep (\<beta> v) i)(x := u i) \<Turnstile> \<phi>)\<close>
+      by (smt (verit, best) F_filter filter.in_F_subset_S mem_Collect_eq)
+    then obtain I' where
+      \<open>I' \<subseteq> I\<close> and
+      \<open>I' \<in> F\<close> and
+      entails_equiv_in_I':
+      \<open>\<forall> i \<in> I'. \<M> i,(\<lambda> v. rep (\<beta> v) i)(x := rep c i) \<Turnstile> \<phi> \<longleftrightarrow>
+        \<M> i,(\<lambda> v. rep (\<beta> v) i)(x := u i) \<Turnstile> \<phi>\<close>
+      by blast
+    then have I'_inter_K_in_F: \<open>I' \<inter> ?K \<in> F\<close>
+      using filter.closed_int[OF F_filter _ ex_unfolded]
+      by blast 
+    then have \<open>\<forall> i \<in> I' \<inter> ?K. \<M> i,(\<lambda> v. rep (\<beta> v) i)(x := rep c i) \<Turnstile> \<phi>\<close>
+      by (simp add: entails_equiv_in_I' u_def) 
+    then have \<open>I' \<inter> ?K \<subseteq> {i \<in> I. \<M> i,(\<lambda> v. rep (\<beta> v) i)(x := rep c i) \<Turnstile> \<phi>}\<close>
+      by blast 
+    then have \<open>{i \<in> I. \<M> i,(\<lambda> v. rep (\<beta> v) i)(x := rep c i) \<Turnstile> \<phi>} \<in> F\<close>
+      using filter.upwards_closed[OF F_filter _ _ I'_inter_K_in_F] CollectD
+      by force
+    then have
+      \<open>\<exists> u \<in> dom \<A>. {i \<in> I. \<M> i,(\<lambda> v. rep (\<beta> v) i)(x := rep u i) \<Turnstile> \<phi>} \<in> F\<close>
+      unfolding c_def
+      using dom_\<A> u_in_dom
+      by (smt (verit, ccfv_SIG) Collect_cong Pi_iff comp_apply quotientI)
+    then have *: \<open>\<exists> u \<in> dom \<A>. {i \<in> I. \<M> i,(\<lambda> v. rep ((\<beta>(x := u)) v) i) \<Turnstile> \<phi>} \<in> F\<close>
+      by (simp add: fun_upd_rep_is_rep_fun_upd)  
+    then have \<open>\<exists> a \<in> dom \<A>. \<A>,\<beta>(x := a) \<Turnstile> \<phi>\<close>
+    proof -
+      obtain u where
+        u_in_A: \<open>u \<in> dom \<A>\<close> and
+        set_in_F: \<open>{i \<in> I. \<M> i,(\<lambda> v. rep ((\<beta>(x := u)) v) i) \<Turnstile> \<phi>} \<in> F\<close>
+        using "*"
+        by blast
+      then have \<open>is_vars (dom \<A>) (\<beta>(x := u))\<close>
+        using Existential.prems
+        by auto
+      then have \<open>\<A>,\<beta>(x := u) \<Turnstile> \<phi>\<close> 
+        using Existential.IH(1) set_in_F 
+        by blast 
+      then show ?thesis
+        using u_in_A
+        by blast 
+    qed
+    then show \<open>\<A>,\<beta> \<Turnstile> (\<^bold>\<exists> x\<^bold>. \<phi>)\<close> 
+      by simp
+  qed
+next
+  case Bot
+
+  have \<open>\<not> (\<A>,\<beta> \<Turnstile> \<^bold>\<bottom>)\<close>
+    by simp 
+  moreover have \<open>I\<^bsub>\<^bold>\<bottom>\<^esub>\<^bsup>\<beta>\<^esup> = {}\<close>
+    by simp 
+  moreover have \<open>{} \<notin> F\<close>
+    using filter.empty_not_in_F[OF F_filter] . 
+  ultimately show ?case
+    by auto 
+qed
+
+end (* locale ultraprod *)
 
 
 
+section \<open>Compactness proof of full first-order logic\<close>
 
+lemma sat_compactness1: \<open>satisfiable T \<Longrightarrow> \<forall> T' \<subseteq> T. finite T' \<longrightarrow> satisfiable T'\<close>
+  using is_model_of_mono satI
+  by blast
 
+abbreviation (input) I_fm2 
+  :: \<open>'i set \<Rightarrow> ('i \<Rightarrow> ('f, 'p, 'm) model) \<Rightarrow> ('i \<Rightarrow> 'v \<Rightarrow> 'm) \<Rightarrow> ('f, 'p, 'v) fm \<Rightarrow> 'i set\<close>
+  (\<open>_\<^bsup>_,_\<^esup>\<^bsub>_\<^esub>\<close>) where
+  \<open>I\<^bsup>\<M>,\<beta>\<^esup>\<^bsub>\<phi>\<^esub> \<equiv> {i \<in> I. \<M> i,\<beta> i \<Turnstile> \<phi>}\<close> 
 
+text \<open>
+  The name of this lemma comes from the drawing:
+  \<^verbatim>\<open>A \<leftrightarrow> B\<newline>\<updown>  \<updown>\<newline>C \<leftrightarrow> D\<close>
+\<close> 
+lemma iff_square: \<open>A \<longleftrightarrow> B \<Longrightarrow> C \<longleftrightarrow> D \<Longrightarrow> B \<longleftrightarrow> D \<Longrightarrow> A \<longleftrightarrow> C\<close>
+  by blast 
 
+lemma sat_compactness2:
+  \<open>\<forall> T' \<subseteq> T. finite T' \<longrightarrow> satisfiable T' \<Longrightarrow> satisfiable T\<close>
+  for
+    T :: \<open>('f, 'p, 'v) fm set\<close> 
+proof (cases \<open>T = {}\<close>) 
+  case True
+  then show ?thesis
+    by (meson emptyE is_model_of_def satI) 
+next
+  case False
 
+  \<comment>\<open>This proof is mostly inspired by the one in
+    \<^url>\<open>https://www.people.vcu.edu/~bmcody/Compactness-Notes.pdf\<close>, although slightly modified here
+    and there.\<close>
 
+  let ?I = \<open>{ T' :: ('f, 'p, 'v) fm set. finite T' \<and> T' \<subseteq> T }\<close>
 
+  have dummy_I_nonempty: \<open>?I \<noteq> {}\<close>
+    using False
+    by blast 
 
+  assume \<open>\<forall> T' \<subseteq> T. finite T' \<longrightarrow> satisfiable T'\<close>
+  then have \<open>\<forall> T' \<in> ?I. satisfiable T'\<close>
+    by blast 
+  then obtain
+    \<M> :: \<open>('f, 'p, 'v) fm set \<Rightarrow> ('f, 'p, ('f, 'v) tm) model\<close> where
+    \<open>\<forall> i \<in> ?I. is_canonical (\<M> i) (language i) \<and> is_model_of (\<M> i) i\<close>
+    by moura
+  then have 
+    all_\<M>_canonical: \<open>\<forall> i \<in> ?I. is_canonical (\<M> i) (language i)\<close> and
+    i_modelled_by: \<open>\<forall> i \<in> ?I. is_model_of (\<M> i) i\<close>
+    by blast+ 
+  then have
+    structs: \<open>\<forall> i \<in> ?I. struct (dom (\<M> i)) (interp_fn (\<M> i)) (interp_rel (\<M> i))\<close>
+    using model_is_struct
+    by blast
 
+  have \<open>\<forall> f. \<forall> i\<^sub>1 \<in> ?I. \<forall> i\<^sub>2 \<in> ?I. interp_fn (\<M> i\<^sub>1) f = interp_fn (\<M> i\<^sub>2) f\<close>
+    using all_\<M>_canonical[unfolded is_canonical_def]
+    by auto 
 
+  let ?\<beta> = \<open>\<lambda> i _. \<some> x. x \<in> dom (\<M> i)\<close>
 
+  have vars: \<open>\<forall> i \<in> ?I. is_vars (dom (\<M> i)) (?\<beta> i)\<close>
+    unfolding is_vars_def
+    using some_in_eq struct.M_nonempty structs
+    by fastforce
 
+  define star where
+    \<open>star \<equiv> \<lambda> i \<in> ?I. {j \<in> ?I. i \<subseteq> j}\<close>
 
+  have star_nonempty: \<open>star i \<noteq> {}\<close>
+    if \<open>i \<in> ?I\<close>
+    for i
+    unfolding star_def
+    using that
+    by auto
 
+  have \<open>fip {star i | i. i \<in> ?I}\<close> (is \<open>fip ?J\<close>)
+    unfolding fip_def 
+  proof (intro allI impI) 
+    fix H
+    assume
+      H_subset: \<open>H \<subseteq> ?J\<close> and
+      H_finite: \<open>finite H\<close> 
 
+    have inter_star_is_star_union: \<open>star i\<^sub>0 \<inter> star i\<^sub>1 = star (i\<^sub>0 \<union> i\<^sub>1)\<close>
+      if
+        \<open>i\<^sub>0 \<in> ?I\<close> and
+        \<open>i\<^sub>1 \<in> ?I\<close>
+      for i\<^sub>0 i\<^sub>1
+    proof -
+      have \<open>star i\<^sub>0 \<inter> star i\<^sub>1 = {j \<in> ?I. i\<^sub>0 \<subseteq> j} \<inter> {j \<in> ?I. i\<^sub>1 \<subseteq> j}\<close>
+        unfolding star_def
+        using that
+        by auto 
+      also have \<open>... = {j \<in> ?I. i\<^sub>0 \<subseteq> j \<and> i\<^sub>1 \<subseteq> j}\<close>
+        by fast 
+      also have \<open>... = {j \<in> ?I. i\<^sub>0 \<union> i\<^sub>1 \<subseteq> j}\<close>
+        by auto 
+      also have \<open>... = star (i\<^sub>0 \<union> i\<^sub>1)\<close>
+        unfolding star_def
+        using that
+        by simp 
+      finally show ?thesis .
+    qed
+    moreover have \<open>star (i\<^sub>0 \<union> i\<^sub>1) \<noteq> {}\<close>
+      if
+        \<open>i\<^sub>0 \<in> ?I\<close> and
+        \<open>i\<^sub>1 \<in> ?I\<close>
+      for i\<^sub>0 i\<^sub>1
+      using star_nonempty that
+      by auto
+    ultimately have inter_star_nonempty: \<open>star i\<^sub>0 \<inter> star i\<^sub>1 \<noteq> {}\<close>
+      if
+        \<open>i\<^sub>0 \<in> ?I\<close> and
+        \<open>i\<^sub>1 \<in> ?I\<close>
+      for i\<^sub>0 i\<^sub>1
+      using that
+      by auto 
 
-theorem sat_compactness': \<open>sat m T \<longleftrightarrow> (\<exists> T' \<subseteq> T. sat m T')\<close>
-  using sat_compactness
-  sorry 
+    have \<open>\<forall> i \<in> H. \<exists> x \<in> ?I. i = star x\<close>
+      using H_subset
+      by blast 
+    then obtain f where
+      all_in_H_is_star: \<open>\<forall> i \<in> H. f i \<in> ?I \<and> i = star (f i)\<close>
+      by moura 
+
+    have \<open>\<exists> i \<in> ?I. \<Inter> H = star i\<close>
+      if \<open>H \<noteq> {}\<close>
+      using H_subset all_in_H_is_star
+    proof (induction rule: finite_ne_induct[OF H_finite that])
+      case insert: (2 x F)
+      then obtain i\<^sub>0 where
+        i\<^sub>0_in_dummy_I: \<open>i\<^sub>0 \<in> ?I\<close> and
+        \<open>\<Inter> F = star i\<^sub>0\<close>
+        by auto 
+      moreover obtain i\<^sub>1 where
+        i\<^sub>1_in_dummy_I: \<open>i\<^sub>1 \<in> ?I\<close> and
+        \<open>x = star i\<^sub>1\<close>
+        using insert.prems(2)
+        by auto
+      ultimately have
+        \<open>x \<inter> \<Inter> F = star (i\<^sub>1 \<union> i\<^sub>0)\<close>
+        using inter_star_is_star_union
+        by auto 
+      moreover have \<open>i\<^sub>1 \<union> i\<^sub>0 \<in> ?I\<close>
+        using i\<^sub>0_in_dummy_I i\<^sub>1_in_dummy_I
+        by blast 
+      ultimately show ?case
+        by auto 
+    qed auto 
+    then show \<open>\<Inter> H \<noteq> {}\<close>
+      by (cases \<open>H = {}\<close>; fastforce simp: star_nonempty)
+  qed
+  moreover have \<open>?J \<subseteq> Pow ?I\<close>
+    unfolding star_def
+    by auto 
+  ultimately obtain F where
+    \<open>filter F ?I\<close> and
+    dummy_J_subset: \<open>?J \<subseteq> F\<close>
+    using fip_to_filter[OF dummy_I_nonempty, of ?J]
+    by blast 
+  then obtain F' where
+    F'_ultrafilter: \<open>ultrafilter F' ?I\<close> and
+    F_subset: \<open>F \<subseteq> F'\<close>
+    using filter_to_ultrafilter[of F ?I]
+    by blast 
+
+  interpret ultraprod ?I F' \<M> ?\<beta>
+    unfolding ultraprod_def
+    using F'_ultrafilter structs vars
+    by blast 
+
+  {
+    fix \<phi> and \<beta> :: \<open>'v \<Rightarrow> _ set\<close> 
+    assume
+      \<open>\<phi> \<in> T\<close> and
+      vars: \<open>is_vars (dom \<A>) \<beta>\<close> 
+    then have
+      singleton_\<phi>_in_dummy_I: \<open>{\<phi>} \<in> ?I\<close> and
+      \<open>\<forall> i \<in> ?I. \<phi> \<in> i \<longrightarrow> \<M> i,(\<lambda> v. rep (\<beta> v) i) \<Turnstile> \<phi>\<close>
+    proof (blast, intro ballI impI)
+      fix i
+      assume
+        i_in_dummy_I: \<open>i \<in> ?I\<close> and
+        \<phi>_in_i: \<open>\<phi> \<in> i\<close> and
+        \<phi>_in_T: \<open>\<phi> \<in> T\<close>
+
+      have \<open>\<forall> \<beta>. is_vars (dom (\<M> i)) \<beta> \<longrightarrow> \<M> i,\<beta> \<Turnstile> \<phi>\<close>
+        using \<phi>_in_i i_in_dummy_I i_modelled_by is_model_of_def
+        by blast
+      then show \<open>\<M> i,(\<lambda> v. rep (\<beta> v) i) \<Turnstile> \<phi>\<close>
+        using vars dom_\<A> i_in_dummy_I rep_def some_i_in_Mi
+        by auto
+    qed
+    then have \<open>{i \<in> ?I. \<phi> \<in> i} \<subseteq> {i \<in> ?I. \<M> i,(\<lambda> v. rep (\<beta> v) i) \<Turnstile> \<phi>}\<close>
+      by blast 
+    moreover have \<open>{i \<in> ?I. \<phi> \<in> i} \<in> ?J\<close>
+    proof -
+      have \<open>{i \<in> ?I. \<phi> \<in> i} = {i \<in> ?I. {\<phi>} \<subseteq> i}\<close>
+        by simp
+      moreover have \<open>{i \<in> ?I. {\<phi>} \<subseteq> i} = star {\<phi>}\<close>
+        unfolding star_def
+        using singleton_\<phi>_in_dummy_I
+        by simp 
+      then have \<open>{i \<in> ?I. {\<phi>} \<subseteq> i} \<in> ?J\<close>
+        using singleton_\<phi>_in_dummy_I
+        by blast 
+      ultimately show ?thesis
+        by argo
+    qed
+    then have \<open>{i \<in> ?I. \<phi> \<in> i} \<in> F'\<close>
+      using F_subset dummy_J_subset
+      by fastforce 
+    ultimately have \<open>{i \<in> ?I. \<M> i,(\<lambda> v. rep (\<beta> v) i) \<Turnstile> \<phi>} \<in> F'\<close>
+      using filter.upwards_closed[OF ultrafilter_is_filter[OF F'_ultrafilter]]
+      by (metis (mono_tags, lifting) mem_Collect_eq subsetI) 
+    then have \<open>\<A>,\<beta> \<Turnstile> \<phi>\<close>
+      unfolding los[OF vars] .
+  }
+  then have \<open>is_model_of \<A> T\<close>
+    unfolding is_model_of_def
+    by blast
+  then show ?thesis  
+    using satI
+    by blast 
+qed
+
+(* Theorem 1.6 and 3.2 *)
+theorem sat_compactness: \<open>satisfiable T \<longleftrightarrow> (\<forall> T' \<subseteq> T. finite T' \<longrightarrow> satisfiable T')\<close>
+  using sat_compactness1 sat_compactness2
+  by blast 
    
 end (* theory *) 
